Core/Eval/Soundness.lean
@@ -64,35 +64,35 @@ theorem get_instance_sound {G : List Global} :
    get_instance x cs G = some ⟨i, _, p, t⟩ ->
    G[i]? = some (Global.inst x p t)
 := by
-intro h
-unfold get_instance at h; simp at h
-generalize fdef : get_instance_from_idx x cs G = f at *
-generalize odef : instance_idx? x cs G = o at *
-cases o <;> simp at *
-case _ i =>
-unfold instance_idx? at odef;
-rw[List.findIdx?_eq_some_iff_getElem] at odef;
-rcases odef with ⟨i_le, odef1, odef2⟩
-split at odef1
-case _ g n y p a e =>
-  unfold get_instance_from_idx at fdef;
-  have lem := check_instance_eq_sound odef1
-  rcases lem with ⟨e1, e2⟩; subst e1; subst e2
-  simp at fdef; rw[<-fdef] at h; simp at h;
-  rw[List.getElem_eq_iff] at e;
-  rw[e] at h; simp at h;
-  rcases h with ⟨h1, h2⟩
-  clear odef1
-  rcases h2 with ⟨e1, e2, e3, e4⟩
-  subst e2; subst e3; simp at e4; rcases e4 with ⟨e4, e5⟩
-  subst e4; subst e5; apply e
-· cases odef1
+ intro h
+ unfold get_instance at h; simp at h
+ generalize fdef : get_instance_from_idx x cs G = f at *
+ generalize odef : instance_idx? x cs G = o at *
+ cases o <;> simp at *
+ case _ i =>
+ unfold instance_idx? at odef;
+ rw[List.findIdx?_eq_some_iff_getElem] at odef;
+ rcases odef with ⟨i_le, odef1, odef2⟩
+ split at odef1
+ case _ g n y p a e =>
+   unfold get_instance_from_idx at fdef;
+   have lem := check_instance_eq_sound odef1
+   rcases lem with ⟨e1, e2⟩; subst e1; subst e2
+   simp at fdef; rw[<-fdef] at h; simp at h;
+   rw[List.getElem_eq_iff] at e;
+   rw[e] at h; simp at h;
+   rcases h with ⟨h1, h2⟩
+   clear odef1
+   rcases h2 with ⟨e1, e2, e3, e4⟩
+   subst e2; subst e3; simp at e4; rcases e4 with ⟨e4, e5⟩
+   subst e4; subst e5; apply e
+ · cases odef1
 
 
 theorem get_match_sound {ctors : Vec Constructor m} {ps : Vec (Pattern m) n}:
   get_match ctors ps = some i ->
   Pattern.Match ctors (ps[i])
- := by
+:= by
  intro h
  unfold get_match at h
  replace h := Vec.findIdx_sound h
@@ -101,133 +101,134 @@ theorem get_match_sound {ctors : Vec Constructor m} {ps : Vec (Pattern m) n}:
 
 theorem eval_sound (Γ : GlobalEnv) :
   M.eval Γ = some N ->
-  Γ ⊢ M ~> N := by
-intro h
-fun_induction Term.eval generalizing N <;> simp at h
-case _ =>  -- lookup defn
-  rw[Option.bind_eq_some_iff] at h; rcases h with ⟨h1, h2, h⟩
-  cases h;
-  apply Red.defn h2
-case _ ih => -- openm
-  rw[Option.bind_eq_some_iff] at h; rcases h with ⟨h1, h2, h⟩
-  rw[Option.bind_eq_some_iff] at h; rcases h with ⟨⟨i, m, p, t⟩, h4, h⟩
-  simp at h; rcases h with ⟨⟨e1, h5⟩, h⟩
-  subst e1;
-  replace h2 := Term.is_data_sound h2
-  replace h4 := get_instance_sound h4
-  replace h5 := pattern_match_sound (cs := h1) (ps := p) h5
-  simp at h5
-  apply Red.openm_match (i := i) (b := t) (b' := N)
-  · apply h2
-  · apply h4
-  · apply h5
-  · simp; symm at h; apply h
+  Γ ⊢ M ~> N
+:= by
+ intro h
+ fun_induction Term.eval generalizing N <;> simp at h
+ case _ =>  -- lookup defn
+   rw[Option.bind_eq_some_iff] at h; rcases h with ⟨h1, h2, h⟩
+   cases h;
+   apply Red.defn h2
+ case _ ih => -- openm
+   rw[Option.bind_eq_some_iff] at h; rcases h with ⟨h1, h2, h⟩
+   rw[Option.bind_eq_some_iff] at h; rcases h with ⟨⟨i, m, p, t⟩, h4, h⟩
+   simp at h; rcases h with ⟨⟨e1, h5⟩, h⟩
+   subst e1;
+   replace h2 := Term.is_data_sound h2
+   replace h4 := get_instance_sound h4
+   replace h5 := pattern_match_sound (cs := h1) (ps := p) h5
+   simp at h5
+   apply Red.openm_match (i := i) (b := t) (b' := N)
+   · apply h2
+   · apply h4
+   · apply h5
+   · simp; symm at h; apply h
 
-case _ ss _ i j ih1 ih2 => -- openm
-  rw[Option.bind_eq_some_iff] at h; rcases h with ⟨h1, h2, h⟩
-  simp at h; rcases h with ⟨h3, h4⟩
+ case _ ss _ i j ih1 ih2 => -- openm
+   rw[Option.bind_eq_some_iff] at h; rcases h with ⟨h1, h2, h⟩
+   simp at h; rcases h with ⟨h3, h4⟩
 
-  replace j := Vec.findIdx_sound j
-  rw[Option.isSome_iff_exists] at j; rcases j with ⟨t', j⟩
-  rw[h3] at j; simp at j; subst h1
-  replace ih2 := ih2 h2
-  replace ih1 := ih1 i h2
-  subst N
-  apply Red.openm_congr i
-  · have e1 := Vec.to_get_elem (ss.to.set i t') i
-    have e2 := Vec.get_set_eq (a := t') (v := ss.to) (i := i)
-    rw[e1, e2]; apply ih1
-  · intro j h;
-    replace h : i ≠ j := by grind
-    have lem := Vec.get_set_neq h (a := t') (v := ss.to)
-    symm at lem
-    simp [<-Vec.to_get_elem] at lem; apply lem
-
-
-case _ ih => -- mtch
-  rw[Option.bind_eq_some_iff] at h; rcases h with ⟨h1, h2, h⟩
-  rw[Option.bind_eq_some_iff] at h; rcases h with ⟨i, h4, h⟩
-  simp at h; symm at h
-  replace h2 := Term.is_data_sound h2
-  replace h4 := get_match_sound h4; rw[<-Fun.Vec.to_get_elem] at h4
-  apply Red.data_match (i := i)
-  · apply h2
-  · apply h4
-  · apply h
-
-case _ ss _ _ m_ss i j ih1 ih2 => -- mtch congr
-  rw[Option.bind_eq_some_iff] at h; rcases h with ⟨h1, h2, h⟩
-  simp at h; subst h
-  replace ih2 := ih2 h2
-  apply Red.match_congr
-  · have e1 := Vec.to_get_elem (ss.to.set i h1) i;
-    have e2 := Vec.get_set_eq (a := h1) (v := ss.to) (i := i)
-    rw[e1, e2]; apply ih2
-  · intro j h;
-    replace h : i ≠ j := by grind
-    have lem := Vec.get_set_neq h (a := h1) (v := ss.to)
-    symm at lem; simp [<-Vec.to_get_elem] at lem; apply lem
+   replace j := Vec.findIdx_sound j
+   rw[Option.isSome_iff_exists] at j; rcases j with ⟨t', j⟩
+   rw[h3] at j; simp at j; subst h1
+   replace ih2 := ih2 h2
+   replace ih1 := ih1 i h2
+   subst N
+   apply Red.openm_congr i
+   · have e1 := Vec.to_get_elem (ss.to.set i t') i
+     have e2 := Vec.get_set_eq (a := t') (v := ss.to) (i := i)
+     rw[e1, e2]; apply ih1
+   · intro j h;
+     replace h : i ≠ j := by grind
+     have lem := Vec.get_set_neq h (a := t') (v := ss.to)
+     symm at lem
+     simp [<-Vec.to_get_elem] at lem; apply lem
 
 
-case _ => -- Λ[K] t •[T]
-  subst N; constructor
+ case _ ih => -- mtch
+   rw[Option.bind_eq_some_iff] at h; rcases h with ⟨h1, h2, h⟩
+   rw[Option.bind_eq_some_iff] at h; rcases h with ⟨i, h4, h⟩
+   simp at h; symm at h
+   replace h2 := Term.is_data_sound h2
+   replace h4 := get_match_sound h4; rw[<-Fun.Vec.to_get_elem] at h4
+   apply Red.data_match (i := i)
+   · apply h2
+   · apply h4
+   · apply h
 
-case _ ih => -- t •[T]
-  rw[Option.bind_eq_some_iff] at h; rcases h with ⟨h1, h2, h⟩
-  simp at h; subst N
-  constructor; apply ih h2
-
-case _ => -- prj 0 app
-  subst N; apply Red.prj_fst_app
-
-case _ => -- prj0 ->
-  subst N; apply Red.prj_fst_arr
-
-case _ => -- prj 1 app
-  subst h
-  apply Red.prj_snd_app
-
-case _ => -- prj 1 arrow
-  subst h
-  apply Red.prj_snd_arr
-
-case _ ih => -- prj congr
-  rw[Option.bind_eq_some_iff] at h; rcases h with ⟨t', h1, h⟩
-  simp at h; subst N
-  replace ih := ih h1
-  apply Red.ctor1_congr ih
-
-case _ => -- β
-  subst N
-  apply Red.beta
-
-case _ ih1 => -- t1 • t2 ~> t1' • t2
-  rw[Option.bind_eq_some_iff] at h; rcases h with ⟨t', h2, h⟩
-  simp at h; subst N
-  replace ih1 := ih1 h2
-  apply Red.app_congr ih1
-
-case _ => -- ∀c[refl] •c[refl]
-  subst h; apply Red.apptc
-
-case _ ih =>
-  subst N
-  apply Red.apptc_congr2;
-  apply ih; assumption
-
-case _ ih =>
-  subst h;
-  apply Red.apptc_congr1
-  apply ih; assumption
+ case _ ss _ _ m_ss i j ih1 ih2 => -- mtch congr
+   rw[Option.bind_eq_some_iff] at h; rcases h with ⟨h1, h2, h⟩
+   simp at h; subst h
+   replace ih2 := ih2 h2
+   apply Red.match_congr
+   · have e1 := Vec.to_get_elem (ss.to.set i h1) i;
+     have e2 := Vec.get_set_eq (a := h1) (v := ss.to) (i := i)
+     rw[e1, e2]; apply ih2
+   · intro j h;
+     replace h : i ≠ j := by grind
+     have lem := Vec.get_set_neq h (a := h1) (v := ss.to)
+     symm at lem; simp [<-Vec.to_get_elem] at lem; apply lem
 
 
-case _ => -- t ▸ refl A ~> t
-  subst h
-  constructor
+ case _ => -- Λ[K] t •[T]
+   subst N; constructor
 
-case _ ih =>
-  rw[Option.bind_eq_some_iff] at h; rcases h with ⟨h1, h2, h⟩
-  simp at h; subst N
-  apply Red.cast_congr; apply ih h2
+ case _ ih => -- t •[T]
+   rw[Option.bind_eq_some_iff] at h; rcases h with ⟨h1, h2, h⟩
+   simp at h; subst N
+   constructor; apply ih h2
+
+ case _ => -- prj 0 app
+   subst N; apply Red.prj_fst_app
+
+ case _ => -- prj0 ->
+   subst N; apply Red.prj_fst_arr
+
+ case _ => -- prj 1 app
+   subst h
+   apply Red.prj_snd_app
+
+ case _ => -- prj 1 arrow
+   subst h
+   apply Red.prj_snd_arr
+
+ case _ ih => -- prj congr
+   rw[Option.bind_eq_some_iff] at h; rcases h with ⟨t', h1, h⟩
+   simp at h; subst N
+   replace ih := ih h1
+   apply Red.ctor1_congr ih
+
+ case _ => -- β
+   subst N
+   apply Red.beta
+
+ case _ ih1 => -- t1 • t2 ~> t1' • t2
+   rw[Option.bind_eq_some_iff] at h; rcases h with ⟨t', h2, h⟩
+   simp at h; subst N
+   replace ih1 := ih1 h2
+   apply Red.app_congr ih1
+
+ case _ => -- ∀c[refl] •c[refl]
+   subst h; apply Red.apptc
+
+ case _ ih =>
+   subst N
+   apply Red.apptc_congr2;
+   apply ih; assumption
+
+ case _ ih =>
+   subst h;
+   apply Red.apptc_congr1
+   apply ih; assumption
+
+
+ case _ => -- t ▸ refl A ~> t
+   subst h
+   constructor
+
+ case _ ih =>
+   rw[Option.bind_eq_some_iff] at h; rcases h with ⟨h1, h2, h⟩
+   simp at h; subst N
+   apply Red.cast_congr; apply ih h2
 
 end Core
