Core/Infer/Exhaustiveness.lean
@@ -22,14 +22,14 @@ theorem ctor_data_linked {ctors : Vec _ n} {T : String} {spTy : SpineTy}{Tys : L
   spTy.return_type.spine = some (T, Tys) ->
   ∃ i : Fin n, ctors[i].1 = c
 := by
-intro wf h1 h2 h3
-replace h2 := EntryWf.from_lookup wf h2
-cases h2; case _ i h2 h3 h4 h5 =>
-cases h4; case _ h4 _ h6 =>
-simp at h6; simp [Ty.is_data] at h4; rw[h6] at h4; simp at h4; subst T
-rw[h2] at h1; simp at h1; rcases h1 with ⟨e1, e2, e3⟩;
-subst e1; subst e2; replace e3 := eq_of_heq e3; subst e3;
-exists i; rw[h3]
+  intro wf h1 h2 h3
+  replace h2 := EntryWf.from_lookup wf h2
+  cases h2; case _ i h2 h3 h4 h5 =>
+  cases h4; case _ h4 _ h6 =>
+  simp at h6; simp [Ty.is_data] at h4; rw[h6] at h4; simp at h4; subst T
+  rw[h2] at h1; simp at h1; rcases h1 with ⟨e1, e2, e3⟩;
+  subst e1; subst e2; replace e3 := eq_of_heq e3; subst e3;
+  exists i; rw[h3]
 
 
 theorem lookup_odata_entry_exists {G : GlobalEnv}:
@@ -37,15 +37,15 @@ theorem lookup_odata_entry_exists {G : GlobalEnv}:
   R.spine = some (T, Tys) ->
   ∃ K, lookup T G = some (Entry.odata T K)
 := by
-intro h1 h2
-unfold Ty.data? at h1; rw[h2] at h1; simp at h1;
-unfold is_data at h1;
-generalize zdef : lookup T G = z at *
-cases z; simp at h1
-case _ e =>
-simp at h1; cases e <;> simp [Entry.is_data] at *
-have lem := lookup_name_agrees zdef; subst lem;
-simp [Entry.name]
+  intro h1 h2
+  unfold Ty.data? at h1; rw[h2] at h1; simp at h1;
+  unfold is_data at h1;
+  generalize zdef : lookup T G = z at *
+  cases z; simp at h1
+  case _ e =>
+  simp at h1; cases e <;> simp [Entry.is_data] at *
+  have lem := lookup_name_agrees zdef; subst lem;
+  simp [Entry.name]
 
 theorem octor_odata_linked {T : String} {spTy : SpineTy}{Tys1 : List Ty}:
   ⊢ G ->
@@ -54,115 +54,115 @@ theorem octor_odata_linked {T : String} {spTy : SpineTy}{Tys1 : List Ty}:
   lookup_octors T G = some ctors ->
   ∃ i : Nat, ctors[i]? = some c
 := by
-intro wf h2 h3 h4
-replace h2 := EntryWf.from_lookup wf h2
-cases h2; case _ h2 h6 =>
-cases h2; simp at h3;
-case _ h7 _ =>
-have lem := lookup_odata_entry_exists h7 h3
-rcases lem with ⟨K, lem⟩
-case _ m1 m2 n Δ R Ks1 Ks2 Ts a1 a2 a3 a4 =>
-clear a4 h7 a3 a2 a1;
-unfold lookup_octors at h4;
-simp at h4;
-induction G generalizing ctors
-simp at h4; subst h4; simp [lookup] at h6
-case _ hd tl ih =>
-cases hd <;> simp at h4
-case octor =>
-  rw[Option.bind_eq_some_iff] at h4; rcases h4 with ⟨ctors', h4, h5⟩
-  rw[Option.bind_eq_some_iff] at h5; rcases h5 with ⟨⟨R', _⟩, h5, h6⟩
-  split at h6;
-  case _ e =>
-    subst e; simp at h6; subst ctors;
-    simp at *;
-    cases wf; case _ wftl wfhd =>
-    unfold lookup at h6;  simp at h6
-    split at h6
-    case _ e => subst e; simp at h6; subst h6; exists 0
-    simp [lookup] at lem;
-    split at lem;
-    case _ e => subst e; simp at lem
-    unfold lookup_octors at h4; simp at h4
-    replace ih := ih wftl h6 lem h4
-    rcases ih with ⟨i, ih⟩; exists i + 1
-  case _ e' =>
-    simp at h6; subst ctors';
-    unfold lookup at h6; simp at h6;
+  intro wf h2 h3 h4
+  replace h2 := EntryWf.from_lookup wf h2
+  cases h2; case _ h2 h6 =>
+  cases h2; simp at h3;
+  case _ h7 _ =>
+  have lem := lookup_odata_entry_exists h7 h3
+  rcases lem with ⟨K, lem⟩
+  case _ m1 m2 n Δ R Ks1 Ks2 Ts a1 a2 a3 a4 =>
+  clear a4 h7 a3 a2 a1;
+  unfold lookup_octors at h4;
+  simp at h4;
+  induction G generalizing ctors
+  simp at h4; subst h4; simp [lookup] at h6
+  case _ hd tl ih =>
+  cases hd <;> simp at h4
+  case octor =>
+    rw[Option.bind_eq_some_iff] at h4; rcases h4 with ⟨ctors', h4, h5⟩
+    rw[Option.bind_eq_some_iff] at h5; rcases h5 with ⟨⟨R', _⟩, h5, h6⟩
     split at h6;
     case _ e =>
-      subst e; simp at h6; subst h6;
-      simp at *
-      simp [lookup] at lem;
-      split at lem
-      case _ e => subst e; simp at  lem
+      subst e; simp at h6; subst ctors;
+      simp at *;
       cases wf; case _ wftl wfhd =>
-      rw[h3] at h5; simp at h5; rcases h5 with ⟨h5, _⟩; symm at h5; contradiction
-    cases wf; case _ wftl wfhd =>
-    simp [lookup] at lem
-    split at lem
-    case _ e => subst e; simp at lem
-    unfold lookup_octors at h4; simp at h4
-    have ih := ih wftl h6 lem h4; apply ih
+      unfold lookup at h6;  simp at h6
+      split at h6
+      case _ e => subst e; simp at h6; subst h6; exists 0
+      simp [lookup] at lem;
+      split at lem;
+      case _ e => subst e; simp at lem
+      unfold lookup_octors at h4; simp at h4
+      replace ih := ih wftl h6 lem h4
+      rcases ih with ⟨i, ih⟩; exists i + 1
+    case _ e' =>
+      simp at h6; subst ctors';
+      unfold lookup at h6; simp at h6;
+      split at h6;
+      case _ e =>
+        subst e; simp at h6; subst h6;
+        simp at *
+        simp [lookup] at lem;
+        split at lem
+        case _ e => subst e; simp at  lem
+        cases wf; case _ wftl wfhd =>
+        rw[h3] at h5; simp at h5; rcases h5 with ⟨h5, _⟩; symm at h5; contradiction
+      cases wf; case _ wftl wfhd =>
+      simp [lookup] at lem
+      split at lem
+      case _ e => subst e; simp at lem
+      unfold lookup_octors at h4; simp at h4
+      have ih := ih wftl h6 lem h4; apply ih
 
-case data =>
-  cases wf; case _ wftl wfhd =>
-  simp [lookup] at h6;
-  split at h6;
-  case _ e => subst e; simp at h6
-  replace h6 := Vec.fold_or h6
-  cases h6;
-  case _ h6 =>
-    simp [lookup] at lem
-    split at lem
-    · case _ e =>
-      subst e; simp at lem
-    · replace lem := Vec.fold_or lem;
-      cases lem
-      case _ lem =>
+  case data =>
+    cases wf; case _ wftl wfhd =>
+    simp [lookup] at h6;
+    split at h6;
+    case _ e => subst e; simp at h6
+    replace h6 := Vec.fold_or h6
+    cases h6;
+    case _ h6 =>
+      simp [lookup] at lem
+      split at lem
+      · case _ e =>
+        subst e; simp at lem
+      · replace lem := Vec.fold_or lem;
+        cases lem
+        case _ lem =>
+          unfold lookup_octors at h4; simp at h4
+          apply ih wftl h6 lem h4
+        case _ e => simp at e
+    case _ h6 => simp at h6
+  case odata =>
+    cases wf; case _ wftl wfhd =>
+    simp [lookup] at h6;
+    split at h6;
+    case _ e =>
+      subst e; simp at h6
+    case _ =>
+      simp [lookup] at lem;
+      split at lem;
+      case _ e =>
+        simp at lem; subst e; simp at lem; subst lem
+        cases wfhd; case _ e =>
+        rw[e] at ih; simp at ih; exfalso
+        have lem := EntryWf.from_lookup wftl h6
+        cases lem; case _ lem _ =>
+        cases lem; case _ h =>
+        unfold Ty.data? at h; simp [h3] at h
+        unfold is_data at h; simp [e] at h;
+      case _ =>
         unfold lookup_octors at h4; simp at h4
         apply ih wftl h6 lem h4
-      case _ e => simp at e
-  case _ h6 => simp at h6
-case odata =>
-  cases wf; case _ wftl wfhd =>
-  simp [lookup] at h6;
-  split at h6;
-  case _ e =>
-    subst e; simp at h6
+  all_goals try (
   case _ =>
+    cases wf; case _ wftl wfhd =>
+    simp [lookup] at h6;
+    split at h6;
+    case _ e =>  simp at h6
     simp [lookup] at lem;
     split at lem;
     case _ e =>
-       simp at lem; subst e; simp at lem; subst lem
-       cases wfhd; case _ e =>
-       rw[e] at ih; simp at ih; exfalso
-       have lem := EntryWf.from_lookup wftl h6
-       cases lem; case _ lem _ =>
-       cases lem; case _ h =>
-       unfold Ty.data? at h; simp [h3] at h
-       unfold is_data at h; simp [e] at h;
-    case _ =>
-      unfold lookup_octors at h4; simp at h4
-      apply ih wftl h6 lem h4
-all_goals try (
-case _ =>
-  cases wf; case _ wftl wfhd =>
-  simp [lookup] at h6;
-  split at h6;
-  case _ e =>  simp at h6
-  simp [lookup] at lem;
-  split at lem;
-  case _ e =>
-    subst e; simp at lem
-  unfold lookup_octors at h4; simp at h4
-  apply ih wftl h6 lem h4)
+      subst e; simp at lem
+    unfold lookup_octors at h4; simp at h4
+    apply ih wftl h6 lem h4)
 
-case inst =>
-  cases wf; case _ wftl wfhd =>
-  simp [lookup] at h6;   simp [lookup] at lem;
-  unfold lookup_octors at h4; simp at h4
-  apply ih wftl h6 lem h4
+  case inst =>
+    cases wf; case _ wftl wfhd =>
+    simp [lookup] at h6;   simp [lookup] at lem;
+    unfold lookup_octors at h4; simp at h4
+    apply ih wftl h6 lem h4
 
 
 theorem lookup_data_entry_exists {G : GlobalEnv}:
@@ -170,15 +170,15 @@ theorem lookup_data_entry_exists {G : GlobalEnv}:
   R.spine = some (T, Tys) ->
   ∃ (K : Kind) (n : Nat) (ctors : Vec (String × SpineTy) n), lookup T G = some (Entry.data (n := n) T K ctors)
 := by
-intro h1 h2
-unfold Ty.data? at h1; rw[h2] at h1; simp at h1;
-unfold is_data at h1;
-generalize zdef : lookup T G = z at *
-cases z; simp at h1
-case _ e =>
-simp at h1; cases e <;> simp [Entry.is_data] at *
-have lem := lookup_name_agrees zdef; subst lem;
-simp [Entry.name]
+  intro h1 h2
+  unfold Ty.data? at h1; rw[h2] at h1; simp at h1;
+  unfold is_data at h1;
+  generalize zdef : lookup T G = z at *
+  cases z; simp at h1
+  case _ e =>
+  simp at h1; cases e <;> simp [Entry.is_data] at *
+  have lem := lookup_name_agrees zdef; subst lem;
+  simp [Entry.name]
 
 
 
@@ -188,12 +188,12 @@ theorem lookup_octor_return_type_entry :
   spTy.return_type.spine = some (T, Tys) ->
   ∃ K, lookup T G = some (Entry.odata T K)
 := by
-intro wf h1 h2
-replace h1 := EntryWf.from_lookup wf h1
-cases h1; case _ h3 h1 =>
-cases h3; case _ h4 _ =>
-simp at h2;
-apply lookup_odata_entry_exists h4 h2
+  intro wf h1 h2
+  replace h1 := EntryWf.from_lookup wf h1
+  cases h1; case _ h3 h1 =>
+  cases h3; case _ h4 _ =>
+  simp at h2;
+  apply lookup_odata_entry_exists h4 h2
 
 
 theorem lookup_ctor_return_type_entry :
@@ -202,13 +202,13 @@ theorem lookup_ctor_return_type_entry :
   spTy.return_type.spine = some (T, Tys) ->
   ∃ (K : Kind) (n : Nat) (ctors : Vec (String × SpineTy) n), lookup T G = some (Entry.data (n := n) T K ctors)
 := by
-intro wf h1 h2
-replace h1 := EntryWf.from_lookup wf h1
-cases h1; case _ h3 h1 =>
-cases h3; case _ n _ K ctors _ lk _ _ _ _ _ _ _ _ _ _ _ h5 h4 _ =>
-simp at h2;
-unfold Ty.is_data at h5; rw[h2] at h5; simp at h5
-subst h5; exists K; exists n; exists ctors
+  intro wf h1 h2
+  replace h1 := EntryWf.from_lookup wf h1
+  cases h1; case _ h3 h1 =>
+  cases h3; case _ n _ K ctors _ lk _ _ _ _ _ _ _ _ _ _ _ h5 h4 _ =>
+  simp at h2;
+  unfold Ty.is_data at h5; rw[h2] at h5; simp at h5
+  subst h5; exists K; exists n; exists ctors
 
 
 theorem lookup_entry_ctor? :
@@ -217,20 +217,20 @@ theorem lookup_entry_ctor? :
  Entry.ctor? d dc ent = true ->
  ∃ c' K spTy tys, (ent = Entry.ctor c' K spTy ∨ ent = Entry.octor c' spTy) ∧ spTy.return_type.spine = some ⟨d, tys⟩
 := by
-intro wf h1 h2
-unfold Entry.ctor? at h2
-have lem := lookup_name_agrees h1; simp [Entry.name] at lem; subst lem
-split at h2 <;> simp at *
-case _ c K _ _ _ _ _ _ _ =>
-  exists c; exists K; simp;
-  split at h2
-  case _ sp _ => simp at h2; subst d; exists sp
-  · cases h2
-case _ c _ _ _ _ T sp _ =>
-  exists c; simp;
-  split at h2
-  case _ sp _ => simp at h2; subst d; exists sp
-  case _ => cases h2
+  intro wf h1 h2
+  unfold Entry.ctor? at h2
+  have lem := lookup_name_agrees h1; simp [Entry.name] at lem; subst lem
+  split at h2 <;> simp at *
+  case _ c K _ _ _ _ _ _ _ =>
+    exists c; exists K; simp;
+    split at h2
+    case _ sp _ => simp at h2; subst d; exists sp
+    · cases h2
+  case _ c _ _ _ _ T sp _ =>
+    exists c; simp;
+    split at h2
+    case _ sp _ => simp at h2; subst d; exists sp
+    case _ => cases h2
 
 
 theorem lookup_ctor_names_sound :
@@ -238,70 +238,70 @@ theorem lookup_ctor_names_sound :
   lookup_ctor? G dc c T = true ->
   lookup_ctor_names G T = some ⟨n, cs⟩ ->
   ∃ j : Fin n, cs[j] = c := by
-intro wf h1 h2
-unfold lookup_ctor? at h1
-unfold lookup_ctor_names at h2; simp at h2
-rw[Option.bind_eq_some_iff] at h2; rcases h2 with ⟨⟨Tx, Targs⟩, h4, h2⟩
-split at h1
-· simp at h2;
-  rw[Option.getD_eq_iff] at h1; simp at h1
-  rcases h1 with ⟨ent, h1, h3⟩
-  split at h2
-  case _ h0 _ _ _ _ _ h2 =>
-    simp at h2; rcases h2 with ⟨e1, e2⟩;
-    subst e1; replace e2 := eq_of_heq e2; simp at *
-    have lem := lookup_name_agrees h1
-    subst e2; simp
-    replace h3 := lookup_entry_ctor? wf h1 h3; rcases h3 with ⟨c', K, spTy, tys, e, e2⟩
-    cases e
-    case _ e =>
-      subst e; simp [Entry.name] at lem; subst c';
-      have lem := lookup_name_agrees h2; simp [Entry.name] at lem; subst lem
-      rw[h0] at h4; simp at h4; obtain ⟨e1, e2⟩ := h4
-      subst e1; subst e2;
-      have lem := ctor_data_linked wf h2 h1 e2
-      apply lem
-    case _ e =>
-      subst e; simp [Entry.name] at lem; subst c';
-      have lem := lookup_name_agrees h2; simp [Entry.name] at lem; subst lem
-      rw[h0] at h4; simp at h4; obtain ⟨e1, e2⟩ := h4
-      subst e1; subst e2;
-      exfalso;
-      have lem := lookup_octor_return_type_entry wf h1 e2
-      rcases lem with ⟨K, lem⟩; rw[lem] at h2; simp at h2
+  intro wf h1 h2
+  unfold lookup_ctor? at h1
+  unfold lookup_ctor_names at h2; simp at h2
+  rw[Option.bind_eq_some_iff] at h2; rcases h2 with ⟨⟨Tx, Targs⟩, h4, h2⟩
+  split at h1
+  · simp at h2;
+    rw[Option.getD_eq_iff] at h1; simp at h1
+    rcases h1 with ⟨ent, h1, h3⟩
+    split at h2
+    case _ h0 _ _ _ _ _ h2 =>
+      simp at h2; rcases h2 with ⟨e1, e2⟩;
+      subst e1; replace e2 := eq_of_heq e2;
+      have lem := lookup_name_agrees h1
+      subst e2; simp
+      replace h3 := lookup_entry_ctor? wf h1 h3; rcases h3 with ⟨c', K, spTy, tys, e, e2⟩
+      cases e
+      case _ e =>
+        subst e; simp [Entry.name] at lem; subst c';
+        have lem := lookup_name_agrees h2; simp [Entry.name] at lem; subst lem
+        rw[h0] at h4; simp at h4; obtain ⟨e1, e2⟩ := h4
+        subst e1; subst e2;
+        have lem := ctor_data_linked wf h2 h1 e2
+        apply lem
+      case _ e =>
+        subst e; simp [Entry.name] at lem; subst c';
+        have lem := lookup_name_agrees h2; simp [Entry.name] at lem; subst lem
+        rw[h0] at h4; simp at h4; obtain ⟨e1, e2⟩ := h4
+        subst e1; subst e2;
+        exfalso;
+        have lem := lookup_octor_return_type_entry wf h1 e2
+        rcases lem with ⟨K, lem⟩; rw[lem] at h2; simp at h2
 
-  case _ h4 =>
-    rw[Option.bind_eq_some_iff] at h2; rcases h2 with ⟨cs, h2, h5⟩
-    have lem := lookup_name_agrees h4; simp [Entry.name] at lem; subst lem;
-    case _ tsp2 _ _ _  tsp1 =>
-    rw[tsp1] at tsp2; simp at tsp2; rcases tsp2 with ⟨e1, e2⟩; subst e1; subst e2
-    have lem := lookup_entry_ctor? wf h1 h3
-    rcases lem with ⟨c1, K, spTy, Tys1, ch, Tys2⟩
-    cases ch
-    case _ ch =>
-      subst ch;
-      have lem := lookup_name_agrees h1; simp [Entry.name] at lem; subst lem;
-      exfalso;
-      unfold Entry.ctor? at h3;
-      split at h3;
-      · case _ e =>
-          simp at e; rcases e with ⟨e1, e2, e3⟩; subst e1; subst e2; subst e3; simp at *;
-          rw[Tys2] at h3; simp at h3; clear h3;
-          have lem := lookup_ctor_return_type_entry wf h1 Tys2
-          rcases lem with ⟨K, n, ctors, lem⟩
-          rw[lem] at h4; simp at h4
-      · case _ e => simp at e
-      · cases h3
+    case _ h4 =>
+      rw[Option.bind_eq_some_iff] at h2; rcases h2 with ⟨cs, h2, h5⟩
+      have lem := lookup_name_agrees h4; simp [Entry.name] at lem; subst lem;
+      case _ tsp2 _ _ _  tsp1 =>
+      rw[tsp1] at tsp2; simp at tsp2; rcases tsp2 with ⟨e1, e2⟩; subst e1; subst e2
+      have lem := lookup_entry_ctor? wf h1 h3
+      rcases lem with ⟨c1, K, spTy, Tys1, ch, Tys2⟩
+      cases ch
+      case _ ch =>
+        subst ch;
+        have lem := lookup_name_agrees h1; simp [Entry.name] at lem; subst lem;
+        exfalso;
+        unfold Entry.ctor? at h3;
+        split at h3;
+        · case _ e =>
+            simp at e; rcases e with ⟨e1, e2, e3⟩; subst e1; subst e2; subst e3; simp at *;
+            rw[Tys2] at h3; simp at h3; clear h3;
+            have lem := lookup_ctor_return_type_entry wf h1 Tys2
+            rcases lem with ⟨K, n, ctors, lem⟩
+            rw[lem] at h4; simp at h4
+        · case _ e => simp at e
+        · cases h3
 
-    case _ ch =>
-      subst ch
-      have lem := lookup_name_agrees h1; simp [Entry.name] at lem; subst lem;
-      have lem := octor_odata_linked wf h1 Tys2 h2
-      simp at h5; rcases lem with ⟨i, lem⟩
-      apply Vec.from_list_indexing h5 lem
-  cases h2
+      case _ ch =>
+        subst ch
+        have lem := lookup_name_agrees h1; simp [Entry.name] at lem; subst lem;
+        have lem := octor_odata_linked wf h1 Tys2 h2
+        simp at h5; rcases lem with ⟨i, lem⟩
+        apply Vec.from_list_indexing h5 lem
+    cases h2
 
-· cases h1
+  · cases h1
 
 
 -- Given a vector of types, builds a matrix of all possible combination of constructor names
@@ -344,29 +344,29 @@ def patterns_to_ctor_names (ps : Vec (Pattern m) n) : Vec (Vec String m) n :=
 theorem pattern_match_rfl {q : Vec String m} {p : Pattern m} :
   p.to_ctor_names = q <-> Query.Match q p
 := by
-apply Iff.intro
-· intro h
-  induction m <;> simp at *
-  case _ =>
-    unfold Query.Match;
-    cases p; cases q; apply VecTyping.nil
-  case _ ih =>
-    unfold Query.Match
-    cases q; case _ q qs =>
-    cases p; case _ p ps =>
-    simp at h
-    apply VecTyping.cons
-    · exists p.2.1; exists p.2.2.1; exists p.2.2.2
-      rw[<-h.1]
-    apply ih
-    · apply h.2
-· intro h
-  induction h
-  case _ => simp
-  case _ h _ ih =>
-    simp
-    rcases h with ⟨_, _, _, h⟩
-    cases h; simp; apply ih
+  apply Iff.intro
+  · intro h
+    induction m <;> simp at *
+    case _ =>
+      unfold Query.Match;
+      cases p; cases q; apply VecTyping.nil
+    case _ ih =>
+      unfold Query.Match
+      cases q; case _ q qs =>
+      cases p; case _ p ps =>
+      simp at h
+      apply VecTyping.cons
+      · exists p.2.1; exists p.2.2.1; exists p.2.2.2
+        rw[<-h.1]
+      apply ih
+      · apply h.2
+  · intro h
+    induction h
+    case _ => simp
+    case _ h _ ih =>
+      simp
+      rcases h with ⟨_, _, _, h⟩
+      cases h; simp; apply ih
 
 theorem pattern_extension_enumerate {G : GlobalEnv} {S : Ty} :
   ⊢ G ->
@@ -378,25 +378,25 @@ theorem pattern_extension_enumerate {G : GlobalEnv} {S : Ty} :
   Vec.populate (⟨nc, cs⟩ :: ctor_names) = ⟨ℓ', ref_matrix'⟩ ->
   ∀ i : Fin ℓ, ∃ j' : Fin ℓ', ref_matrix'[j'] = y :: ref_matrix[i]
 := by
-intro wf h3 h5 h6 h7 i
-have lem := lookup_ctor_names_sound wf h5 h6
-rcases lem with ⟨k, lem⟩;
-unfold Vec.populate at h7; simp at h7; unfold Vec.populate at h3; rw[h3] at h7
-have comb_size_lem := Vec.combine_size h7; simp at comb_size_lem
-subst ℓ'
-have lem1 := Vec.combine_soundness h7
-simp at lem1;
-replace lem1 := lem1 k i
-rcases lem1 with ⟨j', lem1⟩
-exists j'; rw[lem] at lem1;
-apply Eq.symm lem1
+  intro wf h3 h5 h6 h7 i
+  have lem := lookup_ctor_names_sound wf h5 h6
+  rcases lem with ⟨k, lem⟩;
+  unfold Vec.populate at h7; simp at h7; unfold Vec.populate at h3; rw[h3] at h7
+  have comb_size_lem := Vec.combine_size h7; simp at comb_size_lem
+  subst ℓ'
+  have lem1 := Vec.combine_soundness h7
+  simp at lem1;
+  replace lem1 := lem1 k i
+  rcases lem1 with ⟨j', lem1⟩
+  exists j'; rw[lem] at lem1;
+  apply Eq.symm lem1
 
 
 theorem fin_shift_lemma {bs cs : Vec _ n} :
   (∀ (i : Fin (n + 1)), lookup_ctor_names G (Vec.cons b bs)[i] = some (c :: cs)[i]) ->
   ∀ (i : Fin n), lookup_ctor_names G bs[i] = some cs[i] := by
-intro h i
-replace h := h (i.succ); simp at h; apply h
+  intro h i
+  replace h := h (i.succ); simp at h; apply h
 
 theorem heq_cast_l {a : α} {b : β} {e : α = β} : a ≍ b -> a = (b |> cast (by rw[e]))
 := by subst e; simp;
@@ -415,7 +415,7 @@ theorem cast_cons {a : α} {b : Vec α n} {e : α = β} :
 -- set_option pp.explicit true
 
 theorem cast_sigma (c0 : ((p : Nat) × Vec (Vec String (0 + (x + 1))) p) = ((n : Nat) × Vec (Vec String (x + 1)) n)) : cast c0 ⟨ℓ, z⟩ = ⟨ℓ', z'⟩ -> ℓ = ℓ' ∧ ∃ c, z = cast c z' := by
-intro h; grind;
+  intro h; grind;
 
 @[simp]
 theorem Vec.cast_cons
@@ -445,70 +445,70 @@ theorem query_in_enumerate_ctors {G : GlobalEnv} {q : Vec String m} {S : Vec Ty 
   Query G dc q S ->
   enumerate_ctor_names G S = some ⟨ℓ, ref_matrix⟩ ->
   ∃ j : Fin ℓ, ref_matrix[j] = q := by
-intro wf h1 h2
-unfold enumerate_ctor_names at h2; simp at h2
-rw[Option.bind_eq_some_iff] at h2; rcases h2 with ⟨ctor_names, h3, h2⟩
-injection h2; case _ h2 =>
-replace h3 := Vec.traverse_eq_pure_iff_getElem_Option h3
-unfold Query at h1;
-induction h1 generalizing ℓ <;> simp at *
-case _ =>
-  generalize zdef : Vec.populate_aux ⟨1, #(#())⟩ ctor_names = z at *
-  subst h2; cases ctor_names; simp at zdef;
-  obtain ⟨e1, e2⟩ := zdef; subst e1; replace e2 := eq_of_heq e2; subst e2; simp;
-case _ x _ _ lc _ ih =>
-  generalize zdef : Vec.populate_aux ⟨1, #(#())⟩ ctor_names = z at *
-  cases ctor_names; case _ c cs =>
+  intro wf h1 h2
+  unfold enumerate_ctor_names at h2; simp at h2
+  rw[Option.bind_eq_some_iff] at h2; rcases h2 with ⟨ctor_names, h3, h2⟩
+  injection h2; case _ h2 =>
+  replace h3 := Vec.traverse_eq_pure_iff_getElem_Option h3
+  unfold Query at h1;
+  induction h1 generalizing ℓ <;> try simp at *
+  case _ =>
+    generalize zdef : Vec.populate_aux ⟨1, #(#())⟩ ctor_names = z at *
+    subst h2; cases ctor_names; simp at zdef;
+    obtain ⟨e1, e2⟩ := zdef; subst e1; replace e2 := eq_of_heq e2; subst e2; simp;
+  case _ x _ _ lc _ ih =>
+    generalize zdef : Vec.populate_aux ⟨1, #(#())⟩ ctor_names = z at *
+    cases ctor_names; case _ c cs =>
 
-  have z_size := Vec.populate_size _ zdef
-  simp at z_size;
-  have h3' := fin_shift_lemma h3
-  replace h3 := h3 0; simp at h3
-  have lem := lookup_ctor_names_sound wf lc h3
-  obtain ⟨j, lem⟩ := lem
-  simp at zdef;
-  generalize zdef' : Vec.populate_aux ⟨1, #() :: #()⟩ cs = z' at *
-  rcases z' with ⟨z', z'h⟩
-  rcases z with ⟨z, zh⟩;
+    have z_size := Vec.populate_size _ zdef
+    simp at z_size;
+    have h3' := fin_shift_lemma h3
+    replace h3 := h3 0; simp at h3
+    have lem := lookup_ctor_names_sound wf lc h3
+    obtain ⟨j, lem⟩ := lem
+    simp at zdef;
+    generalize zdef' : Vec.populate_aux ⟨1, #() :: #()⟩ cs = z' at *
+    rcases z' with ⟨z', z'h⟩
+    rcases z with ⟨z, zh⟩;
 
-  have lem2 := Vec.combine_soundness zdef
-  have lem0 : zh ≍ ref_matrix := by grind
-  have lemz : z = ℓ := by grind
-  subst z;
+    have lem2 := Vec.combine_soundness zdef
+    have lem0 : zh ≍ ref_matrix := by grind
+    have lemz : z = ℓ := by grind
+    subst z;
 
-  -- c + z'h = zh ≍ ref_matrix
+    -- c + z'h = zh ≍ ref_matrix
 
-  replace lem2 := lem2 j
+    replace lem2 := lem2 j
 
-  subst lem; simp at lem2
-  simp at z_size; subst ℓ
+    subst lem; simp at lem2
+    simp at z_size; subst ℓ
 
-  replace ih := @ih z' (ref_matrix := z'h |> cast (by rw[Nat.zero_add])) _ (by {
-    rw[zdef']; grind}) h3'
-  rcases ih with ⟨j', ih⟩
-  replace lem2 := lem2 j'
-  rcases lem2 with ⟨j'', lem2⟩
+    replace ih := @ih z' (ref_matrix := z'h |> cast (by rw[Nat.zero_add])) _ (by {
+      rw[zdef']; grind}) h3'
+    rcases ih with ⟨j', ih⟩
+    replace lem2 := lem2 j'
+    rcases lem2 with ⟨j'', lem2⟩
 
-  generalize c0_def : enumerate_ctor_names._proof_1 = c0 at *
+    generalize c0_def : enumerate_ctor_names._proof_1 = c0 at *
 
-  subst ih;
-  exists j''
+    subst ih;
+    exists j''
 
-  have e1 : ref_matrix[j''] = cast (by simp) zh[j''] := by
-    have h := cast_get_elem (e := by rw[Nat.zero_add]) j'' lem0
-    rw[<-h]
-  rw[e1]; rw[<-lem2]; clear lem2; norm_cast;
-  generalize c2_def : of_eq_true
-    (Eq.trans (congrFun' (congrArg Eq (congrArg (Vec String) (Nat.zero_add (x + 1)))) (Vec String (x + 1)))
-      (eq_self (Vec String (x + 1))))  = c2 at *
-  replace h2 := cast_sigma c0 h2;
-  rcases h2 with ⟨_, c3, h3⟩
+    have e1 : ref_matrix[j''] = cast (by simp) zh[j''] := by
+      have h := cast_get_elem (e := by rw[Nat.zero_add]) j'' lem0
+      rw[<-h]
+    rw[e1]; rw[<-lem2]; clear lem2; norm_cast;
+    generalize c2_def : of_eq_true
+      (Eq.trans (congrFun' (congrArg Eq (congrArg (Vec String) (Nat.zero_add (x + 1)))) (Vec String (x + 1)))
+        (eq_self (Vec String (x + 1))))  = c2 at *
+    replace h2 := cast_sigma c0 h2;
+    rcases h2 with ⟨_, c3, h3⟩
 
-  have lem : ∃ c1, cast c2 (c.snd[j] :: z'h[j']) = Vec.cons (c.snd[j]) (cast c1 (z'h[j'])) := by
-    grind
-  rcases lem with ⟨c4, lem⟩
-  rw[lem]; congr;
-  apply cast_indexing
+    have lem : ∃ c1, cast c2 (c.snd[j] :: z'h[j']) = Vec.cons (c.snd[j]) (cast c1 (z'h[j'])) := by
+      grind
+    rcases lem with ⟨c4, lem⟩
+    rw[lem]; congr;
+    apply cast_indexing
 
 
 -- Checks that the patterns are exhaustive
@@ -530,15 +530,15 @@ theorem check_exhaustive_sound {G : GlobalEnv} {q : Vec String m} {S : Vec Ty m}
   Query G dc q S ->
   check_exhaustive G S ps = some ⟨ℓ, ⟨ref_matrix, idxs⟩⟩ ->
   ∃ j : Fin ℓ, ref_matrix[j] = q := by
-intro wf h1 h2
-unfold check_exhaustive at h2; simp at h2
-rw[Option.bind_eq_some_iff] at h2; rcases h2 with ⟨ref_matrix, h4, h2⟩
-rw[Option.bind_eq_some_iff] at h2; rcases h2 with ⟨idxs, h6, h2⟩
-replace h6 := Vec.traverse_eq_pure_iff_getElem_Option h6
-cases h2;
-cases ref_matrix; case _ n ref_matrix =>
-simp at idxs;
-simp at h6; simp
-apply query_in_enumerate_ctors wf h1 h4
+  intro wf h1 h2
+  unfold check_exhaustive at h2; simp at h2
+  rw[Option.bind_eq_some_iff] at h2; rcases h2 with ⟨ref_matrix, h4, h2⟩
+  rw[Option.bind_eq_some_iff] at h2; rcases h2 with ⟨idxs, h6, h2⟩
+  replace h6 := Vec.traverse_eq_pure_iff_getElem_Option h6
+  cases h2;
+  cases ref_matrix; case _ n ref_matrix =>
+  simp at idxs;
+  simp at h6; simp
+  apply query_in_enumerate_ctors wf h1 h4
 
 end Core
