Core/Infer/GlobalSound.lean
@@ -14,136 +14,138 @@ theorem wf_global_sound :
   GlobalEnv.wf_globals G = some () ->
   ⊢ G
 := by
-intro h
-fun_induction GlobalEnv.wf_globals <;> simp at *
-case _ =>  -- empty
-  apply ListGlobalWf.nil
+  intro h
+  fun_induction GlobalEnv.wf_globals <;> simp at *
+  case _ =>  -- empty
+    apply ListGlobalWf.nil
 
-case _ n x k ctors G ih => -- ctors
-  rw[Option.bind_eq_some_iff] at h; rcases h with ⟨h1, h2, h⟩
-  simp at h; rcases h with ⟨h3, h⟩
-  rw[Option.bind_eq_some_iff] at h; rcases h with ⟨h4, h5, h⟩
-  rw[Option.bind_eq_some_iff] at h; rcases h with ⟨h6, h7, h⟩
-  rw[Option.bind_eq_some_iff] at h; rcases h with ⟨h8, h9, h⟩
-  replace h5 := Vec.traverse_eq_pure_iff_getElem_Option h5
-  replace h7 := Vec.traverse_eq_pure_iff_getElem_Option h7
-  replace h9 := Vec.traverse_eq_pure_iff_getElem_Option h9
-  replace h4 := Vec.units h4;
-  rcases h3 with ⟨h3a, h3b⟩
-  replace h3b := Vec.unique_elems_sound h3b;
-  apply ListGlobalWf.cons; simp at h3b
-  · apply GlobalWf.data (G := G) (n := n) (K := k) (x := x) (ctors := ctors)
-    · intro i y T h
-      apply And.intro
-      · replace h5 := h5 i; simp at h5;
-        replace h5 := spine_kinding_sound h5; simp at h5;
-        have lem : ctors[i].1 = y := by rw[h]
-        rw[lem] at h5; clear lem;
-        have lem : ctors[i].2 = T := by rw[h]
-        rw[lem] at h5; apply h5
-      · apply And.intro
-        · replace h7 := h7 i; rw[h] at h7; simp at h7; simp; intro f; apply h7 (Eq.symm f)
-        · replace h9 := h9 i; rw[h] at h9; simp at h9; apply h9
-    · apply h3b
-    · apply h3a
-  · apply ih h2
+  case _ n x k ctors G ih => -- ctors
+    rw[Option.bind_eq_some_iff] at h; rcases h with ⟨h1, h2, h⟩
+    simp at h; rcases h with ⟨h3, h⟩
+    rw[Option.bind_eq_some_iff] at h; rcases h with ⟨h4, h5, h⟩
+    rw[Option.bind_eq_some_iff] at h; rcases h with ⟨h6, h7, h⟩
+    rw[Option.bind_eq_some_iff] at h; rcases h with ⟨h8, h9, h⟩
+    replace h5 := Vec.traverse_eq_pure_iff_getElem_Option h5
+    replace h7 := Vec.traverse_eq_pure_iff_getElem_Option h7
+    replace h9 := Vec.traverse_eq_pure_iff_getElem_Option h9
+    replace h4 := Vec.units h4;
+    rcases h3 with ⟨h3a, h3b⟩
+    replace h3b := Vec.unique_elems_sound h3b;
+    apply ListGlobalWf.cons; simp at h3b
+    · apply GlobalWf.data (G := G) (n := n) (K := k) (x := x) (ctors := ctors)
+      · intro i y T h
+        apply And.intro
+        · replace h5 := h5 i;
+          replace h5 := spine_kinding_sound h5;
+          have lem : ctors[i].1 = y := by rw[h]
+          rw[lem] at h5; clear lem;
+          have lem : ctors[i].2 = T := by rw[h]
+          rw[lem] at h5; apply h5
+        · apply And.intro
+          · replace h7 := h7 i; rw[h] at h7; simp at h7; simp; intro f; apply h7 (Eq.symm f)
+          · replace h9 := h9 i; rw[h] at h9; simp at h9; apply h9
+      · apply h3b
+      · apply h3a
+    · apply ih h2
 
-case _ ih =>  -- openm
-  rw[Option.bind_eq_some_iff] at h; rcases h with ⟨h1, h2, h⟩
-  simp at h;  rcases h with ⟨h3, h⟩
-  replace h := spine_kinding_sound h
-  replace ih := ih h2
-  apply ListGlobalWf.cons
-  · apply GlobalWf.openm h h3
-  · apply ih
-
-case _ ih =>  -- octor
-  rw[Option.bind_eq_some_iff] at h; rcases h with ⟨h1, h2, h⟩
-  simp at h; rcases h with ⟨e, h⟩
-  apply ListGlobalWf.cons
-  · apply GlobalWf.octor
-    apply spine_kinding_sound h
-    apply e
-  · apply ih h2
-
-case _ ih => -- defn
-  rw[Option.bind_eq_some_iff] at h; rcases h with ⟨h1, h2, h⟩
-  rw[Option.bind_eq_some_iff] at h; rcases h with ⟨h3, h4, h⟩
-  rw[Option.bind_eq_some_iff] at h; rcases h with ⟨h5, h6, h⟩
-  rw[Option.bind_eq_some_iff] at h; rcases h with ⟨h7, h8, h⟩
-  simp at h; rcases h with ⟨e1, h⟩; subst e1
-  apply ListGlobalWf.cons
-  · apply GlobalWf.defn
-    · replace h8 := Kind.base_kind_sound _ h8; subst h5
-      replace h6 := infer_kind_sound h6; apply h6
-    · replace h4 := infer_type_sound (ih h2) h4; apply h4
-    · apply h
-  · apply ih h2
-
-case _ m _ p t G ih => -- inst
-  rw[Option.bind_eq_some_iff] at h; rcases h with ⟨h1, h2, h⟩
-  split at h
-  case _ x _ _ _ Ks1 _ Ks2 _ Ts R lk =>
-    simp at h; rcases h with ⟨⟨e1, e2⟩, h⟩; subst e1; subst e2;
-    rw[Option.bind_eq_some_iff] at h; rcases h with ⟨ξ, h4, h⟩
-    rw[Option.bind_eq_some_iff] at h; rcases h with ⟨h5, h6, h⟩
-    simp at h; subst h
+  case _ ih =>  -- openm
+    rw[Option.bind_eq_some_iff] at h; rcases h with ⟨h1, h2, h⟩
+    simp at h;  rcases h with ⟨h3, h⟩
+    replace h := spine_kinding_sound h
     replace ih := ih h2
-    rcases ξ with ⟨Δ', Γ⟩
-    simp at h6;
-    replace h4 := pattern_binders_sound h4
-    replace h6 := infer_type_sound ih h6
     apply ListGlobalWf.cons
-    · apply GlobalWf.inst
-      · apply lk
-      · rfl
-      · simp; apply h4
-      · simp; apply h6
+    · apply GlobalWf.openm h h3
     · apply ih
-  · cases h
 
-case _ ih => -- odata
-  rw[Option.bind_eq_some_iff] at h; rcases h with ⟨h1, h2, h⟩
-  simp at h
-  apply ListGlobalWf.cons
-  · apply GlobalWf.odata h
-  · apply ih h2
+  case _ ih =>  -- octor
+    rw[Option.bind_eq_some_iff] at h; rcases h with ⟨h1, h2, h⟩
+    simp at h; rcases h with ⟨e, h⟩
+    apply ListGlobalWf.cons
+    · apply GlobalWf.octor
+      apply spine_kinding_sound h
+      apply e
+    · apply ih h2
+
+  case _ ih => -- defn
+    rw[Option.bind_eq_some_iff] at h; rcases h with ⟨h1, h2, h⟩
+    rw[Option.bind_eq_some_iff] at h; rcases h with ⟨h3, h4, h⟩
+    rw[Option.bind_eq_some_iff] at h; rcases h with ⟨h5, h6, h⟩
+    rw[Option.bind_eq_some_iff] at h; rcases h with ⟨h7, h8, h⟩
+    simp at h; rcases h with ⟨e1, h⟩; subst e1
+    apply ListGlobalWf.cons
+    · apply GlobalWf.defn
+      · replace h8 := Kind.base_kind_sound _ h8; subst h5
+        replace h6 := infer_kind_sound h6; apply h6
+      · replace h4 := infer_type_sound (ih h2) h4; apply h4
+      · apply h
+    · apply ih h2
+
+  case _ m _ p t G ih => -- inst
+    rw[Option.bind_eq_some_iff] at h; rcases h with ⟨h1, h2, h⟩
+    split at h
+    case _ x _ _ _ Ks1 _ Ks2 _ Ts R lk =>
+      simp at h; rcases h with ⟨⟨e1, e2⟩, h⟩; subst e1; subst e2;
+      rw[Option.bind_eq_some_iff] at h; rcases h with ⟨ξ, h4, h⟩
+      rw[Option.bind_eq_some_iff] at h; rcases h with ⟨h5, h6, h⟩
+      simp at h; subst h
+      replace ih := ih h2
+      rcases ξ with ⟨Δ', Γ⟩
+      simp at h6;
+      replace h4 := pattern_binders_sound h4
+      replace h6 := infer_type_sound ih h6
+      apply ListGlobalWf.cons
+      · apply GlobalWf.inst
+        · apply lk
+        · rfl
+        · simp; apply h4
+        · simp; apply h6
+      · apply ih
+    · cases h
+
+  case _ ih => -- odata
+    rw[Option.bind_eq_some_iff] at h; rcases h with ⟨h1, h2, h⟩
+    simp at h
+    apply ListGlobalWf.cons
+    · apply GlobalWf.odata h
+    · apply ih h2
 
 
 theorem lookup_entry_global {G : GlobalEnv}:
   lookup x G = some (Entry.openm x ⟨na, (Ks1, ⟨nb, (Ks2, ⟨τ, (Ts, R)⟩)⟩)⟩) ->
-  ∃ i : Nat, G[i]? = some (Global.openm x ⟨na, (Ks1, ⟨nb, (Ks2, ⟨τ, (Ts, R)⟩)⟩)⟩) := by
-intro h
-fun_induction lookup <;> simp at *
-case _ ctors _ ctors' ih _ =>
-  replace h := Vec.fold_or h
-  cases h
-  case _ h =>
+  ∃ i : Nat, G[i]? = some (Global.openm x ⟨na, (Ks1, ⟨nb, (Ks2, ⟨τ, (Ts, R)⟩)⟩)⟩)
+:= by
+  intro h
+  fun_induction lookup <;> simp at *
+  case _ ctors _ ctors' ih _ =>
+    replace h := Vec.fold_or h
+    cases h
+    case _ h =>
+      replace ih := ih h
+      rcases ih with ⟨i, ih⟩
+      exists i.succ
+    case _ h =>
+      unfold ctors' at h; simp at h
+  all_goals try (
+    case _ ih _ =>
+    replace ih := ih h
+    rcases ih with ⟨i, ih⟩
+    exists i.succ)
+  case _ =>
+    exists 0; simp; apply h
+  case _ ih =>
     replace ih := ih h
     rcases ih with ⟨i, ih⟩
     exists i.succ
-  case _ h =>
-    unfold ctors' at h; simp at h
-all_goals try (
-  case _ ih _ =>
-  replace ih := ih h
-  rcases ih with ⟨i, ih⟩
-  exists i.succ)
-case _ =>
-  exists 0; simp; apply h
-case _ ih =>
-  replace ih := ih h
-  rcases ih with ⟨i, ih⟩
-  exists i.succ
 
 theorem mk_open_pattern_inversion {g : Global}:
   mk_open_pattern x nc g = some p ->
-  ∃ t, g = .inst x p t := by
-intro h
-unfold mk_open_pattern at h;
-cases g <;> simp at *
-rcases h with ⟨⟨e1, e2⟩, p⟩
-subst e1; subst e2; simp at *; assumption
+  ∃ t, g = .inst x p t
+:= by
+  intro h
+  unfold mk_open_pattern at h;
+  cases g <;> simp at *
+  rcases h with ⟨⟨e1, e2⟩, p⟩
+  subst e1; subst e2; simp at *; assumption
 
 
 theorem mk_open_patterns_inversion {G : GlobalEnv} {ps : List _} :
@@ -160,39 +162,39 @@ theorem open_exhaustive_sound {G : GlobalEnv} :
   G.check_open_exhaustive = some d ->
   OpenExhaustive G
 := by
-intro wf h
-unfold OpenExhaustive
-intro x na nb nc Ks1 Ks2 Ts R q lk qh
-unfold GlobalEnv.check_open_exhaustive at h;
-simp at h;
-replace lk := lookup_entry_global lk
-rcases lk with ⟨oi, lk⟩
-have temp := List.mem_of_getElem? lk
-have h' := h (Global.openm x ⟨na, (Ks1, ⟨nb, (Ks2, ⟨nc, (Ts, R)⟩)⟩)⟩) temp
-unfold GlobalEnv.check_insts at h'
-simp at h'
-rcases h' with ⟨⟨ℓ, ⟨ref_matrix, idxs⟩⟩, h'⟩
-have lem := pattern_exhaustive_sound wf qh h'
-rcases lem with ⟨i, lem⟩;
-generalize zdef : mk_open_patterns G x nc = z at *
-generalize z2def : Vec.from_list z = z2 at *
-rcases z2 with ⟨ℓ', z2⟩
-simp at i;
-have e := Vec.from_list_length z2def
-simp at e; subst e;
-simp at lem; simp at h'; simp at idxs
-have lem1 : z2[i] = z[i] := Vec.from_list_indexing2 z2def i
-rw[lem1] at lem; clear lem1
-have lem3 := mk_open_patterns_inversion zdef z[i] (by simp)
-rcases lem3 with ⟨g, g_in_gs, lem3⟩
-rw[List.mem_iff_getElem?] at g_in_gs
-rcases g_in_gs with ⟨i, g_in_gs⟩
-simp [mk_open_pattern] at lem3
-split at lem3
-case _ j _ _ _ p t =>
-  simp at lem3; rcases lem3 with ⟨⟨e1, e2⟩, lem3⟩
-  subst e1; subst e2; simp at lem3; subst lem3;
-  exists i; exists t; exists z[j]
-· cases lem3
+  intro wf h
+  unfold OpenExhaustive
+  intro x na nb nc Ks1 Ks2 Ts R q lk qh
+  unfold GlobalEnv.check_open_exhaustive at h;
+  simp at h;
+  replace lk := lookup_entry_global lk
+  rcases lk with ⟨oi, lk⟩
+  have temp := List.mem_of_getElem? lk
+  have h' := h (Global.openm x ⟨na, (Ks1, ⟨nb, (Ks2, ⟨nc, (Ts, R)⟩)⟩)⟩) temp
+  unfold GlobalEnv.check_insts at h'
+  simp at h'
+  rcases h' with ⟨⟨ℓ, ⟨ref_matrix, idxs⟩⟩, h'⟩
+  have lem := pattern_exhaustive_sound wf qh h'
+  rcases lem with ⟨i, lem⟩;
+  generalize zdef : mk_open_patterns G x nc = z at *
+  generalize z2def : Vec.from_list z = z2 at *
+  rcases z2 with ⟨ℓ', z2⟩
+  simp at i;
+  have e := Vec.from_list_length z2def
+  subst e;
+  simp at lem; simp at h'; simp at idxs
+  have lem1 : z2[i] = z[i] := Vec.from_list_indexing2 z2def i
+  rw[lem1] at lem; clear lem1
+  have lem3 := mk_open_patterns_inversion zdef z[i] (by simp)
+  rcases lem3 with ⟨g, g_in_gs, lem3⟩
+  rw[List.mem_iff_getElem?] at g_in_gs
+  rcases g_in_gs with ⟨i, g_in_gs⟩
+  simp [mk_open_pattern] at lem3
+  split at lem3
+  case _ j _ _ _ p t =>
+    simp at lem3; rcases lem3 with ⟨⟨e1, e2⟩, lem3⟩
+    subst e1; subst e2; simp at lem3; subst lem3;
+    exists i; exists t; exists z[j]
+  · cases lem3
 
 end Core
