Core/Infer/KindSound.lean
@@ -17,42 +17,42 @@ theorem is_arrow_some : (k : Kind) ->
 
 theorem infer_kind_sound :
   τ.infer_kind G Δ = some k -> G&Δ ⊢ τ : k := by
-intro h
-induction Δ, τ using Ty.infer_kind.induct generalizing k <;> simp at *
-all_goals (try case _ => constructor; assumption)
-case _ ih1 ih2 =>
-  rw[Option.bind_eq_some_iff] at h; rcases h with ⟨_, h1, h⟩
-  rw[Option.bind_eq_some_iff] at h; rcases h with ⟨_, h2, h⟩
-  rw[Option.bind_eq_some_iff] at h; rcases h with ⟨_, h3, h⟩
-  rw[Option.bind_eq_some_iff] at h; rcases h with ⟨_, h4, h⟩
-  simp at h; cases h
-  replace ih1 := ih1 h1
-  replace ih2 := ih2 h3
-  replace h2 := base_kind_some h2
-  replace h4 := base_kind_some h4
-  cases h2; cases h4
-  constructor; assumption; assumption
-case _ ih1 =>
-  rw[Option.bind_eq_some_iff] at h; rcases h with ⟨_, h1, h⟩
-  simp at h; rcases h with ⟨h2, h3⟩
-  subst h2; subst h3
-  replace ih1 := ih1 h1
-  constructor; assumption
-case _ ih1 ih2 =>
-  rw[Option.bind_eq_some_iff] at h; rcases h with ⟨_, h1, h⟩
-  rw[Option.bind_eq_some_iff] at h; rcases h with ⟨_, h2, h⟩
-  simp at h; cases h.1.1; cases h.1.2; cases h.2; clear h
-  have ih1 := ih1 h1
-  have ih2 := ih2 h2
-  constructor; assumption; assumption
-case _ ih1 ih2 =>
-  rw[Option.bind_eq_some_iff] at h; rcases h with ⟨_, h1, h⟩
-  rw[Option.bind_eq_some_iff] at h; rcases h with ⟨_, h2, h⟩
-  rw[Option.bind_eq_some_iff] at h; rcases h with ⟨_, h3, h⟩
-  simp at h; cases h.1; cases h.2; clear h
-  replace h3 := is_arrow_some _ h3; rw[h3] at h1
-  have ih1 := ih1 h1
-  have ih2 := ih2 h2
-  constructor; assumption; assumption
+  intro h
+  induction Δ, τ using Ty.infer_kind.induct generalizing k <;> simp at *
+  all_goals (try case _ => constructor; assumption)
+  case _ ih1 ih2 =>
+    rw[Option.bind_eq_some_iff] at h; rcases h with ⟨_, h1, h⟩
+    rw[Option.bind_eq_some_iff] at h; rcases h with ⟨_, h2, h⟩
+    rw[Option.bind_eq_some_iff] at h; rcases h with ⟨_, h3, h⟩
+    rw[Option.bind_eq_some_iff] at h; rcases h with ⟨_, h4, h⟩
+    simp at h; cases h
+    replace ih1 := ih1 h1
+    replace ih2 := ih2 h3
+    replace h2 := base_kind_some h2
+    replace h4 := base_kind_some h4
+    cases h2; cases h4
+    constructor; assumption; assumption
+  case _ ih1 =>
+    rw[Option.bind_eq_some_iff] at h; rcases h with ⟨_, h1, h⟩
+    simp at h; rcases h with ⟨h2, h3⟩
+    subst h2; subst h3
+    replace ih1 := ih1 h1
+    constructor; assumption
+  case _ ih1 ih2 =>
+    rw[Option.bind_eq_some_iff] at h; rcases h with ⟨_, h1, h⟩
+    rw[Option.bind_eq_some_iff] at h; rcases h with ⟨_, h2, h⟩
+    simp at h; cases h.1.1; cases h.1.2; cases h.2; clear h
+    have ih1 := ih1 h1
+    have ih2 := ih2 h2
+    constructor; assumption; assumption
+  case _ ih1 ih2 =>
+    rw[Option.bind_eq_some_iff] at h; rcases h with ⟨_, h1, h⟩
+    rw[Option.bind_eq_some_iff] at h; rcases h with ⟨_, h2, h⟩
+    rw[Option.bind_eq_some_iff] at h; rcases h with ⟨_, h3, h⟩
+    simp at h; cases h.1; cases h.2; clear h
+    replace h3 := is_arrow_some _ h3; rw[h3] at h1
+    have ih1 := ih1 h1
+    have ih2 := ih2 h2
+    constructor; assumption; assumption
 
 end Core
