Core/Infer/TypeSound.lean
@@ -15,47 +15,49 @@ namespace Core
 
 theorem pattern_binders_sound {v : DataConst} {G : GlobalEnv} {Δ : KindEnv} {m : Nat} {Ts : Vec Ty m} {p : Pattern m}:
   pattern_binders (.data v) G Δ m Ts p = some (ζ, ξ) ->
-  PatternBinders v G Δ m Ts p ζ ξ := by
-intro h
-induction m generalizing ξ ζ <;> simp at *
-case _ =>
-  cases Ts; cases p; cases h
-  case _ e1 e2 =>
-  subst e1; subst e2
-  apply PatternBinders.zero
-case _ n ih =>
-  cases Ts; case _ R' S =>
-  cases p; case _ p ps' =>
-  rcases p with ⟨p1, _, p2, nb, p4⟩
-  unfold pattern_binders at h; simp at h;
-  rw[Option.bind_eq_some_iff] at h; rcases h with ⟨⟨ℓ1, ℓ2⟩, h2, h⟩
-  rw[Option.bind_eq_some_iff] at h; rcases h with ⟨⟨na, Ks1, nb, Ks2, nc, Ts, R⟩, h4, h⟩
-  simp at h; rcases h with ⟨h5, h⟩
-  rw[Option.bind_eq_some_iff] at h; rcases h with ⟨Ks1, h6, h⟩; simp at h
-  rcases h with ⟨h7, h8, h9⟩
-  rcases h9 with ⟨h9, h10⟩; subst h9; subst h10
-  rcases h5 with ⟨⟨e1, e2⟩, e3⟩
-  subst e1; subst e3; subst e2;
-  replace ih := ih h2
-  replace h6 := Vec.traverse_eq_pure_iff_getElem_Option h6
-  replace h7 := Vec.eq_sound_lem h7; simp at h7; subst h7
-  apply PatternBinders.succ
-  · apply h4
-  · intro i; replace h6 := h6 i; replace h6 := infer_kind_sound h6; apply h6
-  · simp;
-  · simp; rfl
-  · simp; apply h8
-  · apply ih
+  PatternBinders v G Δ m Ts p ζ ξ
+:= by
+  intro h
+  induction m generalizing ξ ζ <;> try simp at *
+  case _ =>
+    cases Ts; cases p; cases h
+    case _ e1 e2 =>
+    subst e1; subst e2
+    apply PatternBinders.zero
+  case _ n ih =>
+    cases Ts; case _ R' S =>
+    cases p; case _ p ps' =>
+    rcases p with ⟨p1, _, p2, nb, p4⟩
+    unfold pattern_binders at h; simp at h;
+    rw[Option.bind_eq_some_iff] at h; rcases h with ⟨⟨ℓ1, ℓ2⟩, h2, h⟩
+    rw[Option.bind_eq_some_iff] at h; rcases h with ⟨⟨na, Ks1, nb, Ks2, nc, Ts, R⟩, h4, h⟩
+    simp at h; rcases h with ⟨h5, h⟩
+    rw[Option.bind_eq_some_iff] at h; rcases h with ⟨Ks1, h6, h⟩; simp at h
+    rcases h with ⟨h7, h8, h9⟩
+    rcases h9 with ⟨h9, h10⟩; subst h9; subst h10
+    rcases h5 with ⟨⟨e1, e2⟩, e3⟩
+    subst e1; subst e3; subst e2;
+    replace ih := ih h2
+    replace h6 := Vec.traverse_eq_pure_iff_getElem_Option h6
+    replace h7 := Vec.eq_sound_lem h7; subst h7
+    apply PatternBinders.succ
+    · apply h4
+    · intro i; replace h6 := h6 i; replace h6 := infer_kind_sound h6; apply h6
+    · simp;
+    · simp; rfl
+    · simp; apply h8
+    · apply ih
 
-theorem query_match_sound : query_match q ps = some () -> Query.Match q ps := by
-intro h
-fun_induction query_match <;> simp at *
-case _ a => cases a; apply VecTyping.nil
-case _ y _ ih =>
-  rw[Option.bind_eq_some_iff] at h; rcases h with ⟨h1, h2, h3⟩
-  apply VecTyping.cons
-  simp at h3; exists y.2.1; exists y.2.2.1; exists y.2.2.2; subst h3; rfl
-  apply ih h2
+theorem query_match_sound : query_match q ps = some () -> Query.Match q ps
+:= by
+  intro h
+  fun_induction query_match <;> simp at *
+  case _ a => cases a; apply VecTyping.nil
+  case _ y _ ih =>
+    rw[Option.bind_eq_some_iff] at h; rcases h with ⟨h1, h2, h3⟩
+    apply VecTyping.cons
+    simp at h3; exists y.2.1; exists y.2.2.1; exists y.2.2.2; subst h3; rfl
+    apply ih h2
 
 theorem pattern_exhaustive_sound {G : GlobalEnv} {ps : Vec (Pattern m) k} {q : Vec String m} {S : Vec Ty m} :
   ⊢ G ->
@@ -63,357 +65,359 @@ theorem pattern_exhaustive_sound {G : GlobalEnv} {ps : Vec (Pattern m) k} {q : V
   check_exhaustive G S ps = some ⟨ℓ, ⟨ref_matrix, idxs⟩⟩ ->
   ∃ i : Fin k, Query.Match q ps[i]
 := by
-intro wf h1 h2
-have lem := check_exhaustive_sound wf h1 h2
-unfold check_exhaustive at h2; simp at h2;
-rw[Option.bind_eq_some_iff] at h2; rcases h2 with ⟨ref_matrix, h4, h2⟩
-rw[Option.bind_eq_some_iff] at h2; rcases h2 with ⟨idxs, h6, h2⟩
-replace h6 := Vec.traverse_eq_pure_iff_getElem_Option h6
-cases h2;
-rcases lem with ⟨j, lem⟩
-replace h6 := h6 j;
-replace h6 := Vec.findIdx_sound h6; simp at h6;
-rw[lem] at h6;
-exists idxs[j]
-apply pattern_match_rfl.1 h6
+  intro wf h1 h2
+  have lem := check_exhaustive_sound wf h1 h2
+  unfold check_exhaustive at h2; simp at h2;
+  rw[Option.bind_eq_some_iff] at h2; rcases h2 with ⟨ref_matrix, h4, h2⟩
+  rw[Option.bind_eq_some_iff] at h2; rcases h2 with ⟨idxs, h6, h2⟩
+  replace h6 := Vec.traverse_eq_pure_iff_getElem_Option h6
+  cases h2;
+  rcases lem with ⟨j, lem⟩
+  replace h6 := h6 j;
+  replace h6 := Vec.findIdx_sound h6; simp at h6;
+  rw[lem] at h6;
+  exists idxs[j]
+  apply pattern_match_rfl.1 h6
 
 theorem data_valid_sound (G : GlobalEnv) :
   Ty.valid_data c G T = some () ->
-  T.data? c G := by
-intro h
-induction T <;> simp [Ty.valid_data] at *
-all_goals (assumption)
+  T.data? c G
+:= by
+  intro h
+  induction T <;> simp [Ty.valid_data] at *
+  all_goals (assumption)
 
 theorem spine_kinding_sound :
   spine_kinding G v x test spTy = some () ->
   SpineKinding v x G test spTy
 := by
-intro h
-unfold spine_kinding at h; split at h; simp at h
-case _ Ks1 _ Ks _ _ _ =>
-rw[Option.bind_eq_some_iff] at h; rcases h with ⟨h1, h2, h⟩
-rw[Option.bind_eq_some_iff] at h; rcases h with ⟨h3, h4, h⟩
-simp at h; rcases h with ⟨h5, h⟩
-rcases h5 with ⟨h5, h6⟩; subst h6;
-split at h
-· simp at h;
-  apply SpineKinding.valid (Δ := (Ks1.list ++ Ks.list).reverse)
-  · rfl
-  · intro i; replace h2 := Vec.traverse_eq_pure_iff_getElem_Option h2 i; replace h2 := infer_kind_sound h2;
-    replace h5 := Vec.elems_eq_to_sound h5 i; rw[h5] at h2; simp; apply h2
-  · simp; apply infer_kind_sound h4
-  · apply h
-  · intro h; cases h
+  intro h
+  unfold spine_kinding at h; split at h; simp at h
+  case _ Ks1 _ Ks _ _ _ =>
+  rw[Option.bind_eq_some_iff] at h; rcases h with ⟨h1, h2, h⟩
+  rw[Option.bind_eq_some_iff] at h; rcases h with ⟨h3, h4, h⟩
+  simp at h; rcases h with ⟨h5, h⟩
+  rcases h5 with ⟨h5, h6⟩; subst h6;
+  split at h
+  · simp at h;
+    apply SpineKinding.valid (Δ := (Ks1.list ++ Ks.list).reverse)
+    · rfl
+    · intro i; replace h2 := Vec.traverse_eq_pure_iff_getElem_Option h2 i; replace h2 := infer_kind_sound h2;
+      replace h5 := Vec.elems_eq_to_sound h5 i; rw[h5] at h2; simp; apply h2
+    · simp; apply infer_kind_sound h4
+    · apply h
+    · intro h; cases h
 
-· rw[Option.bind_eq_some_iff] at h; rcases h with ⟨h6, h, _⟩
-  apply SpineKinding.valid (Δ := (Ks1.list ++ Ks.list).reverse)
-  · rfl
-  · intro i; replace h2 := Vec.traverse_eq_pure_iff_getElem_Option h2 i; replace h2 := infer_kind_sound h2;
-    replace h5 := Vec.elems_eq_to_sound h5 i; rw[h5] at h2; simp; apply h2
-  · simp; apply infer_kind_sound h4
-  · simp at *; assumption
-  · intro _ i; replace h := Vec.traverse_eq_pure_iff_getElem_Option h i
-    apply data_valid_sound; replace h6 := Vec.units h6 i; rw[h6] at h
-    apply h
+  · rw[Option.bind_eq_some_iff] at h; rcases h with ⟨h6, h, _⟩
+    apply SpineKinding.valid (Δ := (Ks1.list ++ Ks.list).reverse)
+    · rfl
+    · intro i; replace h2 := Vec.traverse_eq_pure_iff_getElem_Option h2 i; replace h2 := infer_kind_sound h2;
+      replace h5 := Vec.elems_eq_to_sound h5 i; rw[h5] at h2; simp; apply h2
+    · simp; apply infer_kind_sound h4
+    · simp at *; assumption
+    · intro _ i; replace h := Vec.traverse_eq_pure_iff_getElem_Option h i
+      apply data_valid_sound; replace h6 := Vec.units h6 i; rw[h6] at h
+      apply h
 
 theorem infer_type_sound :
   ⊢ G ->
   t.infer_type G Δ Γ = some T ->
-  G&Δ, Γ ⊢ t : T := by
-intro wf h
-fun_induction Term.infer_type generalizing T <;> simp at *
-case _ => -- var
-  rw[Option.bind_eq_some_iff] at h; rcases h with ⟨h1, h2, h⟩
-  rw[Option.bind_eq_some_iff] at h; rcases h with ⟨h3, h4, h⟩
-  rw[Option.bind_eq_some_iff] at h; rcases h with ⟨h5, h6, h⟩
-  cases h
-  replace h6 := Kind.base_kind_sound h3 h6; subst h3
-  apply Typing.var
-  · apply h2
-  · apply infer_kind_sound h4
+  G&Δ, Γ ⊢ t : T
+:= by
+  intro wf h
+  fun_induction Term.infer_type generalizing T <;> simp at *
+  case _ => -- var
+    rw[Option.bind_eq_some_iff] at h; rcases h with ⟨h1, h2, h⟩
+    rw[Option.bind_eq_some_iff] at h; rcases h with ⟨h3, h4, h⟩
+    rw[Option.bind_eq_some_iff] at h; rcases h with ⟨h5, h6, h⟩
+    cases h
+    replace h6 := Kind.base_kind_sound h3 h6; subst h3
+    apply Typing.var
+    · apply h2
+    · apply infer_kind_sound h4
 
-case _ => -- defn
-  rw[Option.bind_eq_some_iff] at h; rcases h with ⟨h1, h2, h⟩
-  rw[Option.bind_eq_some_iff] at h; rcases h with ⟨h3, h4, h⟩; simp at h;
-  rcases h with ⟨h5, h6⟩; subst h3; subst T
-  replace h4 := infer_kind_sound h4
-  apply Typing.defn
-  apply h2
-  apply h4
+  case _ => -- defn
+    rw[Option.bind_eq_some_iff] at h; rcases h with ⟨h1, h2, h⟩
+    rw[Option.bind_eq_some_iff] at h; rcases h with ⟨h3, h4, h⟩; simp at h;
+    rcases h with ⟨h5, h6⟩; subst h3; subst T
+    replace h4 := infer_kind_sound h4
+    apply Typing.defn
+    apply h2
+    apply h4
 
-case _ As _ ih => -- spctor
-  rw[Option.bind_eq_some_iff] at h; rcases h with ⟨⟨m1', Ks1, m2', Ks2, n', Ts, R⟩, h2, h⟩
-  rw[Option.bind_eq_some_iff] at h; rcases h with ⟨Ks1, h4, h⟩;
-  rw[Option.bind_eq_some_iff] at h; rcases h with ⟨Ks, h5, h⟩;
-  simp at h; rcases h with ⟨h5, h⟩
-  rw[Option.bind_eq_some_iff] at h; rcases h with ⟨Ts', h7, h⟩; simp at h
-  rcases h with ⟨h8, h⟩
-  rcases h8 with ⟨⟨⟨h11, h12⟩, h13⟩, h10⟩
-  subst h13;
-  rcases h5 with ⟨⟨⟨e1, e2⟩, e3⟩, h5⟩
-  subst h5; subst e3
-  replace h5 := Vec.traverse_eq_pure_iff_getElem_Option h5
-  replace h4 := Vec.traverse_eq_pure_iff_getElem_Option h4
-  replace e1 := Vec.eq_sound_lem e1; subst Ks1
-  replace e2 := Vec.eq_sound_lem e2; subst Ks
-  replace h12 := Vec.eq_sound_lem h12
-  apply Typing.spctor
-  · rw[h2]
-  · simp; apply Eq.symm h12
-  · simp; apply Eq.symm h
-  · intro i; replace h4 := h4 i; replace h4 := infer_kind_sound h4; apply h4
-  · intro i; replace h5 := h5 i; replace h5 := infer_kind_sound h5; apply h5
-  · intro i; replace h7 := Vec.seq_sound1 _ h7 i;
-    apply ih i; rw[Vec.to_get_elem] at h7; apply h7
-  · intro c e; cases e; apply h11
-  · intro c e; cases e; intro j h; replace h10 := h10 j h; apply Ty.FV.reflection.2 h10
-  · intro h; cases h
+  case _ As _ ih => -- spctor
+    rw[Option.bind_eq_some_iff] at h; rcases h with ⟨⟨m1', Ks1, m2', Ks2, n', Ts, R⟩, h2, h⟩
+    rw[Option.bind_eq_some_iff] at h; rcases h with ⟨Ks1, h4, h⟩;
+    rw[Option.bind_eq_some_iff] at h; rcases h with ⟨Ks, h5, h⟩;
+    simp at h; rcases h with ⟨h5, h⟩
+    rw[Option.bind_eq_some_iff] at h; rcases h with ⟨Ts', h7, h⟩; simp at h
+    rcases h with ⟨h8, h⟩
+    rcases h8 with ⟨⟨⟨h11, h12⟩, h13⟩, h10⟩
+    subst h13;
+    rcases h5 with ⟨⟨⟨e1, e2⟩, e3⟩, h5⟩
+    subst h5; subst e3
+    replace h5 := Vec.traverse_eq_pure_iff_getElem_Option h5
+    replace h4 := Vec.traverse_eq_pure_iff_getElem_Option h4
+    replace e1 := Vec.eq_sound_lem e1; subst Ks1
+    replace e2 := Vec.eq_sound_lem e2; subst Ks
+    replace h12 := Vec.eq_sound_lem h12
+    apply Typing.spctor
+    · rw[h2]
+    · simp; apply Eq.symm h12
+    · simp; apply Eq.symm h
+    · intro i; replace h4 := h4 i; replace h4 := infer_kind_sound h4; apply h4
+    · intro i; replace h5 := h5 i; replace h5 := infer_kind_sound h5; apply h5
+    · intro i; replace h7 := Vec.seq_sound1 _ h7 i;
+      apply ih i; rw[Vec.to_get_elem] at h7; apply h7
+    · intro c e; cases e; apply h11
+    · intro c e; cases e; intro j h; replace h10 := h10 j h; apply Ty.FV.reflection.2 h10
+    · intro h; cases h
 
-case _ As _ ih => -- openm
-  rw[Option.bind_eq_some_iff] at h; rcases h with ⟨h1, h2, h⟩
-  rw[Option.bind_eq_some_iff] at h; rcases h with ⟨Ks1, h4, h⟩
-  rw[Option.bind_eq_some_iff] at h; rcases h with ⟨Ks, h5, h⟩
-  simp at h; rcases h with ⟨h5, h⟩
-  rw[Option.bind_eq_some_iff] at h; rcases h with ⟨Ts', h7, h⟩
-  rw[Option.bind_eq_some_iff] at h; rcases h with ⟨h8, h9, h⟩
-  simp at h; rcases h with ⟨h10, h11⟩
-  rcases h10 with ⟨h10, e⟩; subst e
-  rcases h5 with ⟨⟨⟨e1, e2⟩, e3⟩, e⟩; subst e; subst e3
-  replace e1 := Vec.eq_sound_lem e1; subst Ks1
-  replace e2 := Vec.eq_sound_lem e2; subst e2
-  replace h10 := Vec.eq_sound_lem h10
-  replace h7 := Vec.seq_sound1 _ h7
-  replace h4 := Vec.traverse_eq_pure_iff_getElem_Option h4
-  replace h5 := Vec.traverse_eq_pure_iff_getElem_Option h5
-  replace h9 := Vec.traverse_eq_pure_iff_getElem_Option h9
-  apply Typing.spctor (R := h1.2.2.2.2.2.2) (Ks2 := h1.2.2.2.1) (Ts' := Ts')
-  · rw[h2]
-  · simp; apply Eq.symm h10
-  · simp; apply Eq.symm h11
-  · intro i; replace h4 := h4 i; replace h4 := infer_kind_sound h4; apply h4
-  · intro i; replace h5 := h5 i; replace h5 := infer_kind_sound h5; apply h5
-  · intro i; replace h7 := h7 i; replace ih := @ih i (Ts'.to i) h7; rw[Vec.to_get_elem] at ih; apply ih
-  · intro c e; cases e
-  · intro c e; cases e
-  · intros e i; cases e; replace h9 := h9 i;
-    have lem := Vec.units h8 i; rw[lem] at h9
-    replace h9 := data_valid_sound _ h9; apply h9
+  case _ As _ ih => -- openm
+    rw[Option.bind_eq_some_iff] at h; rcases h with ⟨h1, h2, h⟩
+    rw[Option.bind_eq_some_iff] at h; rcases h with ⟨Ks1, h4, h⟩
+    rw[Option.bind_eq_some_iff] at h; rcases h with ⟨Ks, h5, h⟩
+    simp at h; rcases h with ⟨h5, h⟩
+    rw[Option.bind_eq_some_iff] at h; rcases h with ⟨Ts', h7, h⟩
+    rw[Option.bind_eq_some_iff] at h; rcases h with ⟨h8, h9, h⟩
+    simp at h; rcases h with ⟨h10, h11⟩
+    rcases h10 with ⟨h10, e⟩; subst e
+    rcases h5 with ⟨⟨⟨e1, e2⟩, e3⟩, e⟩; subst e; subst e3
+    replace e1 := Vec.eq_sound_lem e1; subst Ks1
+    replace e2 := Vec.eq_sound_lem e2; subst e2
+    replace h10 := Vec.eq_sound_lem h10
+    replace h7 := Vec.seq_sound1 _ h7
+    replace h4 := Vec.traverse_eq_pure_iff_getElem_Option h4
+    replace h5 := Vec.traverse_eq_pure_iff_getElem_Option h5
+    replace h9 := Vec.traverse_eq_pure_iff_getElem_Option h9
+    apply Typing.spctor (R := h1.2.2.2.2.2.2) (Ks2 := h1.2.2.2.1) (Ts' := Ts')
+    · rw[h2]
+    · simp; apply Eq.symm h10
+    · simp; apply Eq.symm h11
+    · intro i; replace h4 := h4 i; replace h4 := infer_kind_sound h4; apply h4
+    · intro i; replace h5 := h5 i; replace h5 := infer_kind_sound h5; apply h5
+    · intro i; replace h7 := h7 i; replace ih := @ih i (Ts'.to i) h7; rw[Vec.to_get_elem] at ih; apply ih
+    · intro c e; cases e
+    · intro c e; cases e
+    · intros e i; cases e; replace h9 := h9 i;
+      have lem := Vec.units h8 i; rw[lem] at h9
+      replace h9 := data_valid_sound _ h9; apply h9
 
-case _ m n ss ps ts smτs ih1 ih2 => -- match
-  rw[Option.bind_eq_some_iff] at h; rcases h with ⟨S, h2, h⟩
-  rw[Option.bind_eq_some_iff] at h; rcases h with ⟨h3, h4, h⟩
-  rw[Option.bind_eq_some_iff] at h; rcases h with ⟨ζξ, h6, h⟩
-  rw[Option.bind_eq_some_iff] at h; rcases h with ⟨h7, h8, h⟩
-  rw[Option.bind_eq_some_iff] at h; rcases h with ⟨h9, h10, h⟩
-  rw[Option.bind_eq_some_iff] at h; rcases h with ⟨T, h12, h⟩
-  rw[Option.bind_eq_some_iff] at h; rcases h with ⟨_, h13, h⟩
-  cases h;
-  replace h2 := Vec.seq_sound1 _ h2
-  replace h4 := Vec.traverse_eq_pure_iff_getElem_Option h4
-  replace h6 := Vec.seq_sound1 _ h6
-  replace h8 := Vec.seq_sound3 _ h8
-  replace h10 := Vec.traverse_eq_pure_iff_getElem_Option h10
-  replace h12 := Vec.get_elem_if_eq_sound h12
-  let ζ := ζξ.unzip.1
-  let ξ := ζξ.unzip.2
-  apply Typing.mtch (m := m) (n := n) (S := S.to) (ζ := ζ.to) (ξ := ξ.to)
-  · intro i; apply ih1 i (T := S.to i) (h2 i);
-  · intro i; replace h4 := h4 i;
-    have lem := Vec.units h3 i; rw[lem] at h4; rw[Vec.to_get_elem]
-    apply data_valid_sound _ h4
-  · intro i; replace h6 := h6 i;
-    apply pattern_binders_sound;
-    rw[Vec.to_get_elem]; simp; rw[Vec.to_get_elem]; rw[Vec.to_get_elem] at h6; rw[h6]; simp; unfold ζ; unfold ξ;
-    apply Vec.unzip_eta_get_elem -- unzip law
-  · intro i; replace ih2 := @ih2 ζ ξ i (T⟨.add Ty ζ[i].length⟩)
-    rw[Vec.to_get_elem]; rw[Vec.to_get_elem];
-    apply ih2
-    replace h10 := h10 i; simp at h10; rcases h10 with ⟨e1, e2⟩
-    replace h8 := h8 i; simp at h8; unfold ζ; unfold ξ; rw[h8]; rw[Vec.to_get_elem]; simp
-    replace h12 := h12 i; subst T; rw[<-e2]; simp; apply (Eq.symm e1)
-  · intro q qs;
-    rw[<-Vec.to_iso (v := S)] at h13;
-    have lem := pattern_exhaustive_sound wf qs h13
-    rcases lem with ⟨i, lem⟩
-    exists i; rw[Fun.Vec.to_get_elem ps]; apply lem
+  case _ m n ss ps ts smτs ih1 ih2 => -- match
+    rw[Option.bind_eq_some_iff] at h; rcases h with ⟨S, h2, h⟩
+    rw[Option.bind_eq_some_iff] at h; rcases h with ⟨h3, h4, h⟩
+    rw[Option.bind_eq_some_iff] at h; rcases h with ⟨ζξ, h6, h⟩
+    rw[Option.bind_eq_some_iff] at h; rcases h with ⟨h7, h8, h⟩
+    rw[Option.bind_eq_some_iff] at h; rcases h with ⟨h9, h10, h⟩
+    rw[Option.bind_eq_some_iff] at h; rcases h with ⟨T, h12, h⟩
+    rw[Option.bind_eq_some_iff] at h; rcases h with ⟨_, h13, h⟩
+    cases h;
+    replace h2 := Vec.seq_sound1 _ h2
+    replace h4 := Vec.traverse_eq_pure_iff_getElem_Option h4
+    replace h6 := Vec.seq_sound1 _ h6
+    replace h8 := Vec.seq_sound3 _ h8
+    replace h10 := Vec.traverse_eq_pure_iff_getElem_Option h10
+    replace h12 := Vec.get_elem_if_eq_sound h12
+    let ζ := ζξ.unzip.1
+    let ξ := ζξ.unzip.2
+    apply Typing.mtch (m := m) (n := n) (S := S.to) (ζ := ζ.to) (ξ := ξ.to)
+    · intro i; apply ih1 i (T := S.to i) (h2 i);
+    · intro i; replace h4 := h4 i;
+      have lem := Vec.units h3 i; rw[lem] at h4; rw[Vec.to_get_elem]
+      apply data_valid_sound _ h4
+    · intro i; replace h6 := h6 i;
+      apply pattern_binders_sound;
+      rw[Vec.to_get_elem]; simp; rw[Vec.to_get_elem]; rw[Vec.to_get_elem] at h6; rw[h6]; simp; unfold ζ; unfold ξ;
+      apply Vec.unzip_eta_get_elem -- unzip law
+    · intro i; replace ih2 := @ih2 ζ ξ i (T⟨.add Ty ζ[i].length⟩)
+      rw[Vec.to_get_elem]; rw[Vec.to_get_elem];
+      apply ih2
+      replace h10 := h10 i; simp at h10; rcases h10 with ⟨e1, e2⟩
+      replace h8 := h8 i; unfold ζ; unfold ξ; rw[h8]; rw[Vec.to_get_elem]; simp
+      replace h12 := h12 i; subst T; rw[<-e2]; simp; apply (Eq.symm e1)
+    · intro q qs;
+      rw[<-Vec.to_iso (v := S)] at h13;
+      have lem := pattern_exhaustive_sound wf qs h13
+      rcases lem with ⟨i, lem⟩
+      exists i; rw[Fun.Vec.to_get_elem ps]; apply lem
 
-case _ ih1 ih2 => -- cast
-  rw[Option.bind_eq_some_iff] at h; rcases h with ⟨h1, h2, h⟩
-  rw[Option.bind_eq_some_iff] at h; rcases h with ⟨h3, h4, h⟩
-  rw[Option.bind_eq_some_iff] at h; rcases h with ⟨K, h6, h⟩
-  rw[Option.bind_eq_some_iff] at h; rcases h with ⟨h7, h8, h⟩
-  rw[Option.bind_eq_some_iff] at h; rcases h with ⟨h9, h10, h⟩
-  simp at h; rcases h with ⟨h10, h11⟩
-  subst h11; subst h10
-  replace h8 := Kind.base_kind_sound K h8; subst h8
-  replace h4 := Ty.is_eq_some_sound h4; subst h1
-  apply Typing.cast
-  · replace h6 := infer_kind_sound h6
-    apply h6
-  · apply ih1 h2
-  · apply ih2 h10
-  · rfl
+  case _ ih1 ih2 => -- cast
+    rw[Option.bind_eq_some_iff] at h; rcases h with ⟨h1, h2, h⟩
+    rw[Option.bind_eq_some_iff] at h; rcases h with ⟨h3, h4, h⟩
+    rw[Option.bind_eq_some_iff] at h; rcases h with ⟨K, h6, h⟩
+    rw[Option.bind_eq_some_iff] at h; rcases h with ⟨h7, h8, h⟩
+    rw[Option.bind_eq_some_iff] at h; rcases h with ⟨h9, h10, h⟩
+    simp at h; rcases h with ⟨h10, h11⟩
+    subst h11; subst h10
+    replace h8 := Kind.base_kind_sound K h8; subst h8
+    replace h4 := Ty.is_eq_some_sound h4; subst h1
+    apply Typing.cast
+    · replace h6 := infer_kind_sound h6
+      apply h6
+    · apply ih1 h2
+    · apply ih2 h10
+    · rfl
 
-case _ ih => -- lam
-  rw[Option.bind_eq_some_iff] at h; rcases h with ⟨h1, h2, h⟩
-  rw[Option.bind_eq_some_iff] at h; rcases h with ⟨h3, h4, h⟩
-  rw[Option.bind_eq_some_iff] at h; rcases h with ⟨B, h6, h⟩
-  rw[Option.bind_eq_some_iff] at h; rcases h with ⟨h6, h7, h⟩
-  rw[Option.bind_eq_some_iff] at h; rcases h with ⟨h8, h9, h⟩
-  cases h;
-  replace h9 := Kind.base_kind_sound _ h9; subst h6
-  replace h4 := Kind.base_kind_sound _ h4; subst h1
-  apply Typing.lam
-  · apply infer_kind_sound h2
-  · apply ih h6
+  case _ ih => -- lam
+    rw[Option.bind_eq_some_iff] at h; rcases h with ⟨h1, h2, h⟩
+    rw[Option.bind_eq_some_iff] at h; rcases h with ⟨h3, h4, h⟩
+    rw[Option.bind_eq_some_iff] at h; rcases h with ⟨B, h6, h⟩
+    rw[Option.bind_eq_some_iff] at h; rcases h with ⟨h6, h7, h⟩
+    rw[Option.bind_eq_some_iff] at h; rcases h with ⟨h8, h9, h⟩
+    cases h;
+    replace h9 := Kind.base_kind_sound _ h9; subst h6
+    replace h4 := Kind.base_kind_sound _ h4; subst h1
+    apply Typing.lam
+    · apply infer_kind_sound h2
+    · apply ih h6
 
-case _ => -- refl
-  rw[Option.bind_eq_some_iff] at h; rcases h with ⟨h1, h2, h⟩
-  cases h
-  apply Typing.refl
-  · apply infer_kind_sound h2
+  case _ => -- refl
+    rw[Option.bind_eq_some_iff] at h; rcases h with ⟨h1, h2, h⟩
+    cases h
+    apply Typing.refl
+    · apply infer_kind_sound h2
 
-case _ ih => -- t •[T]
-  rw[Option.bind_eq_some_iff] at h; rcases h with ⟨h1, h2, h⟩
-  rw[Option.bind_eq_some_iff] at h; rcases h with ⟨h3, h4, h⟩
-  rw[Option.bind_eq_some_iff] at h; rcases h with ⟨h5, h6, h⟩
-  simp at h; rcases h with ⟨h6, h7⟩
-  subst h1; subst T
-  replace h6 := Ty.is_all_some_sound h6; subst h3
-  apply Typing.appt
-  · apply ih h4
-  · apply infer_kind_sound h2
-  · rfl
+  case _ ih => -- t •[T]
+    rw[Option.bind_eq_some_iff] at h; rcases h with ⟨h1, h2, h⟩
+    rw[Option.bind_eq_some_iff] at h; rcases h with ⟨h3, h4, h⟩
+    rw[Option.bind_eq_some_iff] at h; rcases h with ⟨h5, h6, h⟩
+    simp at h; rcases h with ⟨h6, h7⟩
+    subst h1; subst T
+    replace h6 := Ty.is_all_some_sound h6; subst h3
+    apply Typing.appt
+    · apply ih h4
+    · apply infer_kind_sound h2
+    · rfl
 
-case _ ih => -- prj[0]
-  rw[Option.bind_eq_some_iff] at h; rcases h with ⟨h1, h2, h⟩
-  rw[Option.bind_eq_some_iff] at h; rcases h with ⟨h3, h4, h⟩
-  rw[Option.bind_eq_some_iff] at h; rcases h with ⟨AB, h6, h⟩
-  rw[Option.bind_eq_some_iff] at h; rcases h with ⟨CD, h8, h⟩
-  rw[Option.bind_eq_some_iff] at h; rcases h with ⟨h9, h10, h⟩
-  rw[Option.bind_eq_some_iff] at h; rcases h with ⟨h11, h12, h⟩
-  rw[Option.bind_eq_some_iff] at h; rcases h with ⟨h13, h14, h⟩
-  rw[Option.bind_eq_some_iff] at h; rcases h with ⟨h15, h16, h⟩
-  rw[Option.bind_eq_some_iff] at h; rcases h with ⟨h17, h18, h⟩
-  rw[Option.bind_eq_some_iff] at h; rcases h with ⟨h19, h20, h⟩
-  simp at h;
-  rcases h with ⟨⟨⟨⟨⟨ e5, e6  ⟩, e4⟩, e3⟩, e2⟩ , e1⟩
-  subst e5; subst h13; subst T
-  replace h4 := Ty.is_eq_some_sound h4; subst h1
-  replace h6 := Ty.is_app_some_sound h6
-  replace h8 := Ty.is_app_some_sound h8
-  rw[<-Prod.eta h17] at h18
-  replace h18 := Kind.is_arrow_sound h18
-  subst h9
-  rw[<-Prod.eta h19] at h20
-  replace h20 := Kind.is_arrow_sound h20
-  subst h11
-  apply Typing.prj
-  · apply ih h2
-  · rw[h6, h8, e2]; rw[e2] at h10
-    apply CoercionProject.fst_app
-    · apply infer_kind_sound h10
-    · rcases AB with ⟨A, B⟩; rcases CD with ⟨C,D⟩;
-      rcases h17 with ⟨K1, K2⟩; rcases h19 with ⟨J1, J2⟩;
-      rcases h3 with ⟨K3, H1, H2⟩
-      simp at *; subst e3; subst e6; subst e2; subst H1; subst H2
-      apply infer_kind_sound h12
+  case _ ih => -- prj[0]
+    rw[Option.bind_eq_some_iff] at h; rcases h with ⟨h1, h2, h⟩
+    rw[Option.bind_eq_some_iff] at h; rcases h with ⟨h3, h4, h⟩
+    rw[Option.bind_eq_some_iff] at h; rcases h with ⟨AB, h6, h⟩
+    rw[Option.bind_eq_some_iff] at h; rcases h with ⟨CD, h8, h⟩
+    rw[Option.bind_eq_some_iff] at h; rcases h with ⟨h9, h10, h⟩
+    rw[Option.bind_eq_some_iff] at h; rcases h with ⟨h11, h12, h⟩
+    rw[Option.bind_eq_some_iff] at h; rcases h with ⟨h13, h14, h⟩
+    rw[Option.bind_eq_some_iff] at h; rcases h with ⟨h15, h16, h⟩
+    rw[Option.bind_eq_some_iff] at h; rcases h with ⟨h17, h18, h⟩
+    rw[Option.bind_eq_some_iff] at h; rcases h with ⟨h19, h20, h⟩
+    simp at h;
+    rcases h with ⟨⟨⟨⟨⟨ e5, e6  ⟩, e4⟩, e3⟩, e2⟩ , e1⟩
+    subst e5; subst h13; subst T
+    replace h4 := Ty.is_eq_some_sound h4; subst h1
+    replace h6 := Ty.is_app_some_sound h6
+    replace h8 := Ty.is_app_some_sound h8
+    rw[<-Prod.eta h17] at h18
+    replace h18 := Kind.is_arrow_sound h18
+    subst h9
+    rw[<-Prod.eta h19] at h20
+    replace h20 := Kind.is_arrow_sound h20
+    subst h11
+    apply Typing.prj
+    · apply ih h2
+    · rw[h6, h8, e2]; rw[e2] at h10
+      apply CoercionProject.fst_app
+      · apply infer_kind_sound h10
+      · rcases AB with ⟨A, B⟩; rcases CD with ⟨C,D⟩;
+        rcases h17 with ⟨K1, K2⟩; rcases h19 with ⟨J1, J2⟩;
+        rcases h3 with ⟨K3, H1, H2⟩
+        simp at *; subst e3; subst e6; subst e2; subst H1; subst H2
+        apply infer_kind_sound h12
 
-case _ ih => -- prj[1]
-  rw[Option.bind_eq_some_iff] at h; rcases h with ⟨h1, h2, h⟩
-  rw[Option.bind_eq_some_iff] at h; rcases h with ⟨h3, h4, h⟩
-  rw[Option.bind_eq_some_iff] at h; rcases h with ⟨AB, h6, h⟩
-  rw[Option.bind_eq_some_iff] at h; rcases h with ⟨CD, h8, h⟩
-  rw[Option.bind_eq_some_iff] at h; rcases h with ⟨h9, h10, h⟩
-  rw[Option.bind_eq_some_iff] at h; rcases h with ⟨h11, h12, h⟩
-  rw[Option.bind_eq_some_iff] at h; rcases h with ⟨h13, h14, h⟩
-  rw[Option.bind_eq_some_iff] at h; rcases h with ⟨h15, h16, h⟩
-  rw[Option.bind_eq_some_iff] at h; rcases h with ⟨h17, h18, h⟩
-  rw[Option.bind_eq_some_iff] at h; rcases h with ⟨h19, h20, h⟩
-  simp at h;
-  rcases h with ⟨⟨⟨⟨⟨ e5, e6  ⟩, e4⟩, e3⟩, e2⟩ , e1⟩
-  subst T; subst h13; subst h15
-  rw[e2] at e3;
-  replace h4 := Ty.is_eq_some_sound h4; subst h1
-  replace h6 := Ty.is_app_some_sound h6
-  replace h8 := Ty.is_app_some_sound h8
-  replace h18 := Kind.is_arrow_sound h18; subst h18
-  replace h20 := Kind.is_arrow_sound h20; subst h11
-  apply Typing.prj
-  · apply ih h2
-  · rw[h6, h8];
-    apply CoercionProject.snd_app
-    · apply infer_kind_sound h14
-    · rcases AB with ⟨A, B⟩; rcases CD with ⟨C,D⟩;
-      rcases h17 with ⟨K1, K2⟩; rcases h19 with ⟨J1, J2⟩;
-      rcases h3 with ⟨K3, H1, H2⟩
-      simp at *; subst e3; subst e6; subst e2; subst H1; subst H2
-      apply infer_kind_sound h16
+  case _ ih => -- prj[1]
+    rw[Option.bind_eq_some_iff] at h; rcases h with ⟨h1, h2, h⟩
+    rw[Option.bind_eq_some_iff] at h; rcases h with ⟨h3, h4, h⟩
+    rw[Option.bind_eq_some_iff] at h; rcases h with ⟨AB, h6, h⟩
+    rw[Option.bind_eq_some_iff] at h; rcases h with ⟨CD, h8, h⟩
+    rw[Option.bind_eq_some_iff] at h; rcases h with ⟨h9, h10, h⟩
+    rw[Option.bind_eq_some_iff] at h; rcases h with ⟨h11, h12, h⟩
+    rw[Option.bind_eq_some_iff] at h; rcases h with ⟨h13, h14, h⟩
+    rw[Option.bind_eq_some_iff] at h; rcases h with ⟨h15, h16, h⟩
+    rw[Option.bind_eq_some_iff] at h; rcases h with ⟨h17, h18, h⟩
+    rw[Option.bind_eq_some_iff] at h; rcases h with ⟨h19, h20, h⟩
+    simp at h;
+    rcases h with ⟨⟨⟨⟨⟨ e5, e6  ⟩, e4⟩, e3⟩, e2⟩ , e1⟩
+    subst T; subst h13; subst h15
+    rw[e2] at e3;
+    replace h4 := Ty.is_eq_some_sound h4; subst h1
+    replace h6 := Ty.is_app_some_sound h6
+    replace h8 := Ty.is_app_some_sound h8
+    replace h18 := Kind.is_arrow_sound h18; subst h18
+    replace h20 := Kind.is_arrow_sound h20; subst h11
+    apply Typing.prj
+    · apply ih h2
+    · rw[h6, h8];
+      apply CoercionProject.snd_app
+      · apply infer_kind_sound h14
+      · rcases AB with ⟨A, B⟩; rcases CD with ⟨C,D⟩;
+        rcases h17 with ⟨K1, K2⟩; rcases h19 with ⟨J1, J2⟩;
+        rcases h3 with ⟨K3, H1, H2⟩
+        simp at *; subst e3; subst e6; subst e2; subst H1; subst H2
+        apply infer_kind_sound h16
 
-case _ ih1 ih2 => -- f •c[a]
-  rw[Option.bind_eq_some_iff] at h; rcases h with ⟨h1, h2, h⟩
-  rw[Option.bind_eq_some_iff] at h; rcases h with ⟨h3, h4, h⟩
-  rw[Option.bind_eq_some_iff] at h; rcases h with ⟨h5, h6, h⟩
-  rw[Option.bind_eq_some_iff] at h; rcases h with ⟨h7, h8, h⟩
-  rw[Option.bind_eq_some_iff] at h; rcases h with ⟨h9, h10, h⟩
-  rw[Option.bind_eq_some_iff] at h; rcases h with ⟨h11, h12, h⟩
-  rw[Option.bind_eq_some_iff] at h; rcases h with ⟨h13, h14, h⟩
-  rw[Option.bind_eq_some_iff] at h; rcases h with ⟨h15, h16, h⟩
-  rw[Option.bind_eq_some_iff] at h; rcases h with ⟨h17, h18, h⟩
-  simp at h
-  rcases h with ⟨⟨e1, e2⟩, e3⟩; rw[e1] at e2; subst T
-  replace h6 := Ty.is_eq_some_sound h6; subst h1
-  replace h8 := Kind.base_kind_sound _ h8; rw[h8] at h2; rw[h8] at h4
-  replace h10 := Ty.is_all_some_sound h10; rw[h10] at h2; rw[h10] at h4
-  replace h12 := Ty.is_all_some_sound h12; rw[h12] at h2; rw[h12] at h4
-  replace h18 := Ty.is_eq_some_sound h18; subst h18
-  rw[e1] at h2; rw[e2] at h16; rw[e2] at h14
-  apply Typing.apptc
-  · apply ih1 h2
-  · apply ih2 h14
-  · rfl
-  · rfl
-
-
-case _ ih1 ih2 => -- f • a
-  rw[Option.bind_eq_some_iff] at h; rcases h with ⟨h1, h2, h⟩
-  rw[Option.bind_eq_some_iff] at h; rcases h with ⟨h3, h4, h⟩
-  rw[Option.bind_eq_some_iff] at h; rcases h with ⟨h5, h6, h⟩
-  rw[Option.bind_eq_some_iff] at h; rcases h with ⟨h7, h8, h⟩
-  rw[Option.bind_eq_some_iff] at h; rcases h with ⟨h9, h10, h⟩
-  simp at h; rcases h with ⟨e1, e2⟩
-  subst T; subst h5
-  replace h4 := Ty.is_arrow_some_sound h4; subst h1
-  replace h10 := Kind.base_kind_sound _ h10; subst h7
-  apply Typing.app
-  · apply ih1 h2
-  · apply ih2 h6
+  case _ ih1 ih2 => -- f •c[a]
+    rw[Option.bind_eq_some_iff] at h; rcases h with ⟨h1, h2, h⟩
+    rw[Option.bind_eq_some_iff] at h; rcases h with ⟨h3, h4, h⟩
+    rw[Option.bind_eq_some_iff] at h; rcases h with ⟨h5, h6, h⟩
+    rw[Option.bind_eq_some_iff] at h; rcases h with ⟨h7, h8, h⟩
+    rw[Option.bind_eq_some_iff] at h; rcases h with ⟨h9, h10, h⟩
+    rw[Option.bind_eq_some_iff] at h; rcases h with ⟨h11, h12, h⟩
+    rw[Option.bind_eq_some_iff] at h; rcases h with ⟨h13, h14, h⟩
+    rw[Option.bind_eq_some_iff] at h; rcases h with ⟨h15, h16, h⟩
+    rw[Option.bind_eq_some_iff] at h; rcases h with ⟨h17, h18, h⟩
+    simp at h
+    rcases h with ⟨⟨e1, e2⟩, e3⟩; rw[e1] at e2; subst T
+    replace h6 := Ty.is_eq_some_sound h6; subst h1
+    replace h8 := Kind.base_kind_sound _ h8; rw[h8] at h2; rw[h8] at h4
+    replace h10 := Ty.is_all_some_sound h10; rw[h10] at h2; rw[h10] at h4
+    replace h12 := Ty.is_all_some_sound h12; rw[h12] at h2; rw[h12] at h4
+    replace h18 := Ty.is_eq_some_sound h18; subst h18
+    rw[e1] at h2; rw[e2] at h16; rw[e2] at h14
+    apply Typing.apptc
+    · apply ih1 h2
+    · apply ih2 h14
+    · rfl
+    · rfl
 
 
-case _ ih => -- Λ[K]t
-  rw[Option.bind_eq_some_iff] at h; rcases h with ⟨T, h2, h⟩
-  rw[Option.bind_eq_some_iff] at h; rcases h with ⟨h3, h4, h⟩
-  rw[Option.bind_eq_some_iff] at h; rcases h with ⟨h5, h6, h⟩
-  cases h
-  replace h6 := Kind.base_kind_sound _ h6; subst h3
-  rw[Option.bind_eq_some_iff] at h4; rcases h4 with ⟨h7, h8, h4⟩
-  simp at h4; subst h7
-  apply Typing.lamt
-  · apply Kinding.all
-    · apply infer_kind_sound h8
-  · replace ih := ih h2; simp at ih; apply ih
+  case _ ih1 ih2 => -- f • a
+    rw[Option.bind_eq_some_iff] at h; rcases h with ⟨h1, h2, h⟩
+    rw[Option.bind_eq_some_iff] at h; rcases h with ⟨h3, h4, h⟩
+    rw[Option.bind_eq_some_iff] at h; rcases h with ⟨h5, h6, h⟩
+    rw[Option.bind_eq_some_iff] at h; rcases h with ⟨h7, h8, h⟩
+    rw[Option.bind_eq_some_iff] at h; rcases h with ⟨h9, h10, h⟩
+    simp at h; rcases h with ⟨e1, e2⟩
+    subst T; subst h5
+    replace h4 := Ty.is_arrow_some_sound h4; subst h1
+    replace h10 := Kind.base_kind_sound _ h10; subst h7
+    apply Typing.app
+    · apply ih1 h2
+    · apply ih2 h6
 
-case _ ih => -- ∀c[K]t
-  rw[Option.bind_eq_some_iff] at h; rcases h with ⟨h1, h2, h⟩
-  rw[Option.bind_eq_some_iff] at h; rcases h with ⟨h3, h4, h⟩
-  rw[Option.bind_eq_some_iff] at h; rcases h with ⟨h5, h6, h⟩
-  cases h
-  replace h4 := Ty.is_eq_some_sound h4
-  subst h1
-  replace h6 := Kind.base_kind_sound _ h6
-  rw[h6]; rw[h6] at h2
-  apply Typing.allc
-  · apply ih h2
+
+  case _ ih => -- Λ[K]t
+    rw[Option.bind_eq_some_iff] at h; rcases h with ⟨T, h2, h⟩
+    rw[Option.bind_eq_some_iff] at h; rcases h with ⟨h3, h4, h⟩
+    rw[Option.bind_eq_some_iff] at h; rcases h with ⟨h5, h6, h⟩
+    cases h
+    replace h6 := Kind.base_kind_sound _ h6; subst h3
+    rw[Option.bind_eq_some_iff] at h4; rcases h4 with ⟨h7, h8, h4⟩
+    simp at h4; subst h7
+    apply Typing.lamt
+    · apply Kinding.all
+      · apply infer_kind_sound h8
+    · replace ih := ih h2; apply ih
+
+  case _ ih => -- ∀c[K]t
+    rw[Option.bind_eq_some_iff] at h; rcases h with ⟨h1, h2, h⟩
+    rw[Option.bind_eq_some_iff] at h; rcases h with ⟨h3, h4, h⟩
+    rw[Option.bind_eq_some_iff] at h; rcases h with ⟨h5, h6, h⟩
+    cases h
+    replace h4 := Ty.is_eq_some_sound h4
+    subst h1
+    replace h6 := Kind.base_kind_sound _ h6
+    rw[h6]; rw[h6] at h2
+    apply Typing.allc
+    · apply ih h2
 
 
 end Core
