Core/Ty/Structure.lean
@@ -74,9 +74,9 @@ def Ty.is_all_some : Ty -> Option (Kind × Ty)
 def Ty.is_all_some_sound {T : Ty} :
   T.is_all_some = .some (K, T1) ->
   T = ∀[K] T1 := by
-intro h
-cases T <;> simp [Ty.is_all_some] at *
-assumption
+  intro h
+  cases T <;> simp [Ty.is_all_some] at *
+  assumption
 
 
 def Ty.is_arrow_some : Ty -> Option (Ty × Ty)
@@ -86,9 +86,9 @@ def Ty.is_arrow_some : Ty -> Option (Ty × Ty)
 def Ty.is_arrow_some_sound {T : Ty} :
   T.is_arrow_some = .some (T1, T2) ->
   T = T1 -:> T2 := by
-intro h
-cases T <;> simp [Ty.is_arrow_some] at *
-assumption
+  intro h
+  cases T <;> simp [Ty.is_arrow_some] at *
+  assumption
 
 def Ty.is_eq_some : Ty -> Option (Kind × Ty × Ty)
 | .eq K A B => return (K, A, B)
@@ -97,9 +97,9 @@ def Ty.is_eq_some : Ty -> Option (Kind × Ty × Ty)
 def Ty.is_eq_some_sound {T : Ty} :
   T.is_eq_some = some (K, A, B) ->
   T = (A ~[K]~ B) := by
-intro h;
-cases T <;> simp [Ty.is_eq_some] at *
-assumption
+  intro h;
+  cases T <;> simp [Ty.is_eq_some] at *
+  assumption
 
 def Ty.is_app_some : Ty -> Option (Ty × Ty)
 | .app A B => return (A, B)
@@ -108,9 +108,9 @@ def Ty.is_app_some : Ty -> Option (Ty × Ty)
 def Ty.is_app_some_sound {T : Ty} :
   T.is_app_some = some (A, B) ->
   T = (A • B) := by
-intro h;
-cases T <;> simp [Ty.is_app_some] at *
-assumption
+  intro h;
+  cases T <;> simp [Ty.is_app_some] at *
+  assumption
 
 
 def Ty.subterms : Ty -> List Ty
