Translation/Global/Lemmas.lean
@@ -12,7 +12,7 @@ open Lilac
 
 namespace Core
 
-theorem lookup_append_some {G1 G2 : GlobalEnv} {e : Entry} (wf : ⊢ (G1 ++ G2)):
+theorem lookup_append_some {G1 G2 : List Global} {e : Entry} (wf : ⊢ (G1 ++ G2)):
   Core.lookup x (G1 ++ G2) = some e ->
   Core.lookup x G1 = some e ∨ (Core.lookup x G1 = none ∧ Core.lookup x G2 = some e)
 := by
@@ -20,10 +20,10 @@ theorem lookup_append_some {G1 G2 : GlobalEnv} {e : Entry} (wf : ⊢ (G1 ++ G2))
   induction G1 generalizing G2 x
   · apply Or.inr;
     simp [Core.lookup] at *;
-    have lem : [] ++ G2 = G2 := by grind;
-    simp [lem] at h1; apply h1
-  case _ hd tl ih =>
-    have leme : hd :: tl ++ G2 = hd :: (tl ++ G2) := by grind
+    have lem : [] ++ G2 = G2 := by apply List.nil_append
+    apply h1
+  case _ hd tl ih => -- data
+    have leme : hd :: tl ++ G2 = hd :: (tl ++ G2) := by apply List.cons_append
     rw[leme] at h1;
     cases wf; case _ wftl wfhd =>
     cases hd <;> simp [lookup] at h1
@@ -43,22 +43,36 @@ theorem lookup_append_some {G1 G2 : GlobalEnv} {e : Entry} (wf : ⊢ (G1 ++ G2))
           case _ ih =>
             rcases ih with ⟨ih1, ih2⟩; rw[ih1];
             apply Or.inr; apply And.intro; simp [Vec.fold_or_val_eq_none];
-            · intro v v_in_vs; clear leme; clear lem; clear c1; clear c2
+            · intro v v_in_vs; -- clear leme; clear lem; clear c1; clear c2
               replace v_in_vs := Vec.getElem_of_mem v_in_vs
               rcases v_in_vs with ⟨i, v_in_vs⟩; simp at v_in_vs;
-              replace c3 := c3 i ctors[i].fst ctors[i].snd (by simp)
+              cases leme;
+              replace c3 := c3 i ctors[i].fst ctors[i].snd rfl
               split at v_in_vs;
-              subst x; simp at *; rcases c3 with ⟨_, _, c3⟩; exfalso;
-              sorry
+              subst x; simp at *; subst v; rcases c3 with ⟨_, _, c3⟩; exfalso;
+              simp [c3] at h1;
               symm; apply v_in_vs
             · apply ih2
         case _ h => rcases h with ⟨i, h⟩; apply Or.inl; rw[Vec.foldl_or_eq]; apply Or.inr; exists i
-    sorry
-    sorry
-    sorry
-    sorry
-    sorry
-
+    all_goals try (case _ s _ => -- odata, openm
+      cases wfhd;
+      split at h1;
+      case _ e => subst e; simp at h1; subst e; apply Or.inl; simp [lookup]
+      case _ =>
+        have lem : (x = s) = False := by grind
+        simp [lookup, ite_cond_eq_false (h := lem)]
+        apply ih wftl h1)
+    case _ s _ _ => -- defn, inst
+      cases wfhd; case _ =>
+      split at h1;
+      case _ e => subst e; simp at h1; subst e; apply Or.inl; simp [lookup]
+      case _ =>
+        have lem : (x = s) = False := by grind
+        simp [lookup, ite_cond_eq_false (h := lem)]
+        apply ih wftl h1
+    case _ s _ _ => -- inst
+        simp [lookup]
+        apply ih wftl h1
 
 end Core
 
@@ -103,52 +117,52 @@ theorem Intermediate.Query.opn_strengthen_ctor {Γ : Intermediate.GlobalEnv}
   Intermediate.Query ((Intermediate.Global.data ⟨s, K, ⟨n, ctors⟩⟩ :: Γ)) Intermediate.DataConst.opn q Ts ->
   Intermediate.Query Γ Intermediate.DataConst.opn q Ts
 := by
-intro h
-induction h
-case _ => apply VecTyping.nil
-case _ h1 h2 ih =>
-  apply VecTyping.cons
-  simp [Intermediate.lookup_ctor?] at h1;
-  split at h1 <;> try simp at h1;
-  case _ bsp =>
-    simp [Intermediate.lookup_ctor?]; simp [bsp];
-    simp[Option.getD_eq_iff] at h1; rcases h1 with ⟨ent, lk, h1⟩; simp [Intermediate.lookup] at lk;
-    cases wf; case _ wftl wfhd =>
-    cases wfhd
-    split at lk
-    case _ e => subst e; cases lk; case _ lk _ => exfalso; simp [Intermediate.Entry.ctor?] at h1
-    replace lk := Vec.fold_or lk;
-    cases lk
-    case _ e => simp [e]; apply h1
-    case _ lk =>
-      exfalso
-      rcases lk with ⟨i, lk⟩
-      cases ent <;> simp at *
-      simp [Intermediate.Entry.ctor?] at h1
-  apply ih
+  intro h
+  induction h
+  case _ => apply VecTyping.nil
+  case _ h1 h2 ih =>
+    apply VecTyping.cons
+    simp [Intermediate.lookup_ctor?] at h1;
+    split at h1 <;> try simp at h1;
+    case _ bsp =>
+      simp [Intermediate.lookup_ctor?]; simp [bsp];
+      simp[Option.getD_eq_iff] at h1; rcases h1 with ⟨ent, lk, h1⟩; simp [Intermediate.lookup] at lk;
+      cases wf; case _ wftl wfhd =>
+      cases wfhd
+      split at lk
+      case _ e => subst e; cases lk; case _ lk _ => exfalso; simp [Intermediate.Entry.ctor?] at h1
+      replace lk := Vec.fold_or lk;
+      cases lk
+      case _ e => simp [e]; apply h1
+      case _ lk =>
+        exfalso
+        rcases lk with ⟨i, lk⟩
+        cases ent <;> simp at *
+        simp [Intermediate.Entry.ctor?] at h1
+    apply ih
 
 
 theorem Intermediate.Query.opn_strengthen_defn {Γ : Intermediate.GlobalEnv}
   (wf : ⊢ (Intermediate.Global.defn ⟨s, T, t⟩ :: Γ)) :
   Intermediate.Query ((Intermediate.Global.defn ⟨s, T, t⟩ :: Γ)) Intermediate.DataConst.opn q Ts ->
   Intermediate.Query Γ Intermediate.DataConst.opn q Ts
- := by
-intro h
-induction h
-case _ => apply VecTyping.nil
-case _ h1 h2 ih =>
-  apply VecTyping.cons
-  simp [Intermediate.lookup_ctor?] at h1;
-  split at h1 <;> try simp at h1;
-  case _ bsp =>
-    simp [Intermediate.lookup_ctor?]; simp [bsp];
-    simp[Option.getD_eq_iff] at h1; rcases h1 with ⟨ent, lk, h1⟩; simp [Intermediate.lookup] at lk;
-    cases wf; case _ wftl wfhd =>
-    cases wfhd
-    split at lk
-    case _ e => subst e; cases lk; case _ lk _ => exfalso; simp [Intermediate.Entry.ctor?] at h1
-    simp [lk]; apply h1
-  apply ih
+:= by
+  intro h
+  induction h
+  case _ => apply VecTyping.nil
+  case _ h1 h2 ih =>
+    apply VecTyping.cons
+    simp [Intermediate.lookup_ctor?] at h1;
+    split at h1 <;> try simp at h1;
+    case _ bsp =>
+      simp [Intermediate.lookup_ctor?]; simp [bsp];
+      simp[Option.getD_eq_iff] at h1; rcases h1 with ⟨ent, lk, h1⟩; simp [Intermediate.lookup] at lk;
+      cases wf; case _ wftl wfhd =>
+      cases wfhd
+      split at lk
+      case _ e => subst e; cases lk; case _ lk _ => exfalso; simp [Intermediate.Entry.ctor?] at h1
+      simp [lk]; apply h1
+    apply ih
 
 
 
@@ -157,27 +171,27 @@ theorem Intermediate.Query.opn_strengthen_class {Γ : Intermediate.GlobalEnv}
   Intermediate.Query ((Intermediate.Global.classDecl ⟨s, n, K, fds, scs, mths⟩ :: Γ)) Intermediate.DataConst.opn q Ts ->
   Intermediate.Query Γ Intermediate.DataConst.opn q Ts
 := by
-intro h
-induction h
-case _ => apply VecTyping.nil
-case _ h1 h2 ih =>
-  apply VecTyping.cons
-  simp [Intermediate.lookup_ctor?] at h1;
-  split at h1 <;> try simp at h1;
-  case _ bsp =>
-    simp [Intermediate.lookup_ctor?]; simp [bsp];
-    simp[Option.getD_eq_iff] at h1; rcases h1 with ⟨ent, lk, h1⟩; simp [Intermediate.lookup] at lk;
-    cases wf; case _ wftl wfhd =>
-    cases wfhd
-    split at lk
-    case _ e => subst e; cases lk; case _ lk _ => exfalso; simp [Intermediate.Entry.ctor?] at h1
-    split at lk
-    simp[lk]; apply h1
-    case _ lk1 =>
-    split at lk;
-    cases lk; simp [Intermediate.Entry.ctor?] at h1
-    simp [lk]; apply h1
-  apply ih
+  intro h
+  induction h
+  case _ => apply VecTyping.nil
+  case _ h1 h2 ih =>
+    apply VecTyping.cons
+    simp [Intermediate.lookup_ctor?] at h1;
+    split at h1 <;> try simp at h1;
+    case _ bsp =>
+      simp [Intermediate.lookup_ctor?]; simp [bsp];
+      simp[Option.getD_eq_iff] at h1; rcases h1 with ⟨ent, lk, h1⟩; simp [Intermediate.lookup] at lk;
+      cases wf; case _ wftl wfhd =>
+      cases wfhd
+      split at lk
+      case _ e => subst e; cases lk; case _ lk _ => exfalso; simp [Intermediate.Entry.ctor?] at h1
+      split at lk
+      simp[lk]; apply h1
+      case _ lk1 =>
+      split at lk;
+      cases lk; simp [Intermediate.Entry.ctor?] at h1
+      simp [lk]; apply h1
+    apply ih
 
 
 theorem translate_IC_lookup_some_octor {G : Intermediate.GlobalEnv} {G' : Core.GlobalEnv} (wf : ⊢ G):
@@ -185,133 +199,135 @@ theorem translate_IC_lookup_some_octor {G : Intermediate.GlobalEnv} {G' : Core.G
   Core.lookup x G' = Core.Entry.octor y R ->
   Intermediate.lookup x G = Intermediate.Entry.octor y R
 := by
-intro h1 h2
-fun_induction translate_IC generalizing G' <;> simp at *
-case _ => -- nil
-  simp [pure, Except.pure] at h1; subst G'; simp [Core.lookup] at h2
-case _ ih => -- data
-  simp [Functor.map, Except.map] at h1;
-  split at h1 <;> simp at *
-  subst G'
-  simp [Core.lookup] at h2;
-  split at h2 <;> try simp at *
-  replace h2 := Vec.fold_or h2; cases h2
-  case _ h1 _ h2 =>
+  intro h1 h2
+  fun_induction translate_IC generalizing G' <;> simp at *
+  case _ => -- nil
+    simp [pure, Except.pure] at h1; subst G'; simp [Core.lookup] at h2
+  case _ ih => -- data
+    simp [Functor.map, Except.map] at h1;
+    split at h1 <;> simp at *
+    subst G'
+    simp [Core.lookup] at h2;
+    split at h2 <;> try simp at *
+    replace h2 := Vec.fold_or h2; cases h2
+    case _ h1 _ h2 =>
+      cases wf; case _ wftl wfhd =>
+      simp [Intermediate.lookup]; rw[ite_cond_eq_false (h := by grind)]
+      replace ih := ih wftl h1 h2; rw[ih]
+      rw[Vec.fold_or_val_eq]
+    case _ h =>
+      rcases h with ⟨i, h4⟩; simp at h4
+  case _ ih => -- defn
+    simp [bind, Except.bind] at h1;
+    split at h1 <;> simp at *
+    case _ h3 =>
+    simp [Functor.map, Except.map] at h1
+    split at h1 <;> try simp at h1
+    subst G'; case _ h1 =>
+    simp [Core.lookup] at h2
+    split at h2 <;> try simp at h2
     cases wf; case _ wftl wfhd =>
     simp [Intermediate.lookup]; rw[ite_cond_eq_false (h := by grind)]
-    replace ih := ih wftl h1 h2; rw[ih]
-    rw[Vec.fold_or_val_eq]
-  case _ h =>
-    rcases h with ⟨i, h4⟩; simp at h4
-case _ ih => -- defn
-  simp [bind, Except.bind] at h1;
-  split at h1 <;> simp at *
-  case _ h3 =>
-  simp [Functor.map, Except.map] at h1
-  split at h1 <;> try simp at h1
-  subst G'; case _ h1 =>
-  simp [Core.lookup] at h2
-  split at h2 <;> try simp at h2
-  cases wf; case _ wftl wfhd =>
-  simp [Intermediate.lookup]; rw[ite_cond_eq_false (h := by grind)]
-  apply ih wftl h3 h2
-case _ ih =>   -- class decl
-  simp [Functor.map, Except.map] at h1
-  split at h1 <;> try simp at h1
-  subst G'; case _ h1 =>
-  cases wf; case _ wftl wfhd =>
-    simp [Intermediate.lookup]
+    apply ih wftl h3 h2
+  case _ mths _ ih =>   -- class decl
+    simp [Functor.map, Except.map] at h1
+    split at h1 <;> try simp at h1
+    subst G'; case _ h1 =>
+    cases wf; case _ wftl wfhd =>
+      simp [Intermediate.lookup]
+      split
+      case _ e =>
+        subst e
+        have lem := Core.lookup_name_agrees h2
+        simp [Core.Entry.name] at lem; subst lem
+        cases wfhd
+        generalize G1_def : List.map (fun x => Core.Global.openm x.fst x.snd) mths = G1 at *
+        replace h2 := Core.lookup_append_some (G1 := G1) sorry h2
+        cases h2
+        case _ h2 => sorry
+        case _ h2 =>
+          rcases h2 with ⟨h2, h3⟩
+          sorry
+    -- split
+    -- case _ e =>
+    --   subst e;
+    --   replace h2 := Core.lookup_append h2
+    --   cases h2
+    --   case _ h2 =>
+    --     replace h2 := Core.lookup_append h2
+    --     cases h2
+    --     case _ mths _ _ _ h2 =>
+    --       induction mths <;> simp [Core.lookup] at *
+    --       case _ t ts ih =>
+    --         split at h2 <;> try simp at h2
+    --         apply ih wfhd h2
+    --     case _ h2 =>
+    --       rcases h2 with ⟨_, h2⟩; simp [Core.lookup] at h2
+    --   case _ h2 =>
+    --     rcases h2 with ⟨h2, h3⟩
+    --
+    --     simp [Core.Entry.name] at lem; subst lem;
+
+      sorry
+
+    -- case _ =>
+    --   split
+    --   sorry
+    --   case _ h3 =>
+    --     simp[List.findIdx?_eq_some_iff_getElem] at h3
+    --     rcases h3 with ⟨j, hj, h3⟩
+    --     simp [List.getElem?_eq_getElem (h := j)];
+    --     sorry
+
+  case _ ih => -- inst decl
+    simp [bind, Except.bind] at h1;
+    split at h1 <;> try simp at h1
+    simp [Functor.map, Except.map] at h1
+    split at h1 <;> try simp at h1
+    subst G'
+    case _ h1 _ _ h3 =>
+    simp [Intermediate.lookup];
     split
     case _ e =>
-      subst e
-      have lem := Core.lookup_name_agrees h2
-      simp [Core.Entry.name] at lem; subst lem
-      cases wfhd
-      replace h2 := Core.lookup_append_some sorry h2
-      cases h2
-      case _ h2 => sorry
-      case _ h2 =>
-        rcases h2 with ⟨h2, h3⟩
-        sorry
-  -- split
-  -- case _ e =>
-  --   subst e;
-  --   replace h2 := Core.lookup_append h2
-  --   cases h2
-  --   case _ h2 =>
-  --     replace h2 := Core.lookup_append h2
-  --     cases h2
-  --     case _ mths _ _ _ h2 =>
-  --       induction mths <;> simp [Core.lookup] at *
-  --       case _ t ts ih =>
-  --         split at h2 <;> try simp at h2
-  --         apply ih wfhd h2
-  --     case _ h2 =>
-  --       rcases h2 with ⟨_, h2⟩; simp [Core.lookup] at h2
-  --   case _ h2 =>
-  --     rcases h2 with ⟨h2, h3⟩
-  --
-  --     simp [Core.Entry.name] at lem; subst lem;
-
+      subst e;
+      cases wf; case _ wftl wfhd =>
+      cases wfhd;
+      -- replace h2 := Core.lookup_append  h2
+      -- cases h2
+      -- case _ h2 => sorry
+      sorry
     sorry
-
-  -- case _ =>
-  --   split
-  --   sorry
-  --   case _ h3 =>
-  --     simp[List.findIdx?_eq_some_iff_getElem] at h3
-  --     rcases h3 with ⟨j, hj, h3⟩
-  --     simp [List.getElem?_eq_getElem (h := j)];
-  --     sorry
-
-case _ ih => -- inst decl
-  simp [bind, Except.bind] at h1;
-  split at h1 <;> try simp at h1
-  simp [Functor.map, Except.map] at h1
-  split at h1 <;> try simp at h1
-  subst G'
-  case _ h1 _ _ h3 =>
-  simp [Intermediate.lookup];
-  split
-  case _ e =>
-    subst e;
-    cases wf; case _ wftl wfhd =>
-    cases wfhd;
-    -- replace h2 := Core.lookup_append  h2
-    -- cases h2
-    -- case _ h2 => sorry
-    sorry
-  sorry
 
 theorem mk_inst_mth_SI_sound {Γ' : Intermediate.GlobalEnv} :
   mk_inst_mth_SI Γ' C iname mτs mn tm = .ok i ->
-  ∃ n v na nb, i = ⟨mn, 1, #(⟨iname, n, v, na, nb⟩), tm⟩ := by
-intro h
-unfold mk_inst_mth_SI at h <;> simp at h
-split at h
-case _ h =>
-  split at h <;> try simp [pure, Except.pure, bind, Except.bind_eq_ok_iff] at h;
-  rcases h with ⟨s, h1, b, h2, a1, b1, h3⟩;
-  split at h3 <;> simp at h3
-  subst i;
-  case _ e => rcases e with ⟨e1, e2, e3⟩; subst e1; subst e2; subst e3; simp
-simp at h
+  ∃ n v na nb, i = ⟨mn, 1, #(⟨iname, n, v, na, nb⟩), tm⟩
+:= by
+  intro h
+  unfold mk_inst_mth_SI at h <;> simp at h
+  split at h
+  case _ h =>
+    split at h <;> try simp [pure, Except.pure, bind, Except.bind_eq_ok_iff] at h;
+    rcases h with ⟨s, h1, b, h2, a1, b1, h3⟩;
+    split at h3 <;> simp at h3
+    subst i;
+    case _ e => rcases e with ⟨e1, e2, e3⟩; subst e1; subst e2; subst e3; simp
+  simp at h
 
 theorem mk_inst_mths_SI_sound {Γ' : Intermediate.GlobalEnv} :
   mk_inst_mths_SI Γ' C iname ts mτs = .ok insts ->
   ∀ i ∈ insts, ∃ (mn : String) (n na nb : Nat) (v : Vec Core.Ty n) (t : Surface.Term), i = ⟨mn, 1, #(⟨iname, n, v, na, nb⟩), t⟩
 := by
-intro h p p_in_insts
-fun_induction mk_inst_mths_SI generalizing insts <;> simp [pure, Except.pure] at *
-subst h; simp at p_in_insts
-case _ mn tm ts ih =>
-  simp [bind, Except.bind_eq_ok_iff] at h; rcases h with ⟨insts', h, h1⟩
-  rcases h1 with ⟨mn, b, h1, h2⟩; subst h2
-  simp at p_in_insts; cases p_in_insts
-  case _ h =>
-    subst h; exists mn; replace h1 := mk_inst_mth_SI_sound h1; rcases h1 with ⟨p, h1⟩; simp at h1; rcases h1 with ⟨e, b⟩
-    subst e; rcases b with ⟨n, v, na, nb⟩; subst b; simp
-  case _ h2 => apply ih h h2
+  intro h p p_in_insts
+  fun_induction mk_inst_mths_SI generalizing insts <;> simp [pure, Except.pure] at *
+  subst h; simp at p_in_insts
+  case _ mn tm ts ih =>
+    simp [bind, Except.bind_eq_ok_iff] at h; rcases h with ⟨insts', h, h1⟩
+    rcases h1 with ⟨mn, b, h1, h2⟩; subst h2
+    simp at p_in_insts; cases p_in_insts
+    case _ h =>
+      subst h; exists mn; replace h1 := mk_inst_mth_SI_sound h1; rcases h1 with ⟨p, h1⟩; simp at h1; rcases h1 with ⟨e, b⟩
+      subst e; rcases b with ⟨n, v, na, nb⟩; subst b; simp
+    case _ h2 => apply ih h h2
 
 theorem mk_inst_mths_SI_indexing
 {Γ' : Intermediate.GlobalEnv} :
@@ -365,92 +381,92 @@ theorem translate_SI_lookup_none {G : Surface.GlobalEnv} {G' : Intermediate.Glob
 theorem translate_SI_wf_sound {G : Surface.GlobalEnv} {G' : Intermediate.GlobalEnv} (wf : ⊢ G) :
   ⟦ G ⟧ = .ok G' ->
   ⊢ G' := by
-intro h
-fun_induction translate_SI generalizing G' <;> simp [pure, Except.pure] at *
-case _ =>
-  subst h; constructor
-case _ ctors _ ih =>
-  cases wf; case _ wftl wfhd =>
-  simp [bind, Except.bind_eq_ok_iff] at h; rcases h with ⟨Γ', h1, h⟩
-  split at h <;> simp at h
-  subst G'; case _ h =>
-  rcases h with ⟨h2, h⟩;
-  simp [Vec.all_eq_true] at h;
-  cases wfhd; case _ c1 c2 c3 =>
-  constructor
-  · apply Intermediate.GlobalWf.data
-    · intro i y T h3; replace c3 := c3 i y T h3
-      apply And.intro; sorry; apply And.intro; apply c3.1; sorry
-    · apply c2
-    · apply h2
-  · apply ih wftl h1
-case _ ih => -- defn
-  cases wf; case _ wftl wfhd =>
-  simp [bind, Except.bind_eq_ok_iff] at h; rcases h with ⟨Γ', h1, h⟩
-  split at h <;> simp at h
-  case _ h2 =>
-    subst G'
-    cases wfhd
-    constructor
-    · apply Intermediate.GlobalWf.defn
-      sorry -- needs kind inference defined on Intermediate Global
-      apply h2
-    · apply ih wftl h1
-
-case _ kc s Ks mτs Γ ih =>  -- class decl
-  cases wf; case _ wftl wfhd =>
-  simp [bind, Except.bind_eq_ok_iff] at h; rcases h with ⟨Γ', h1, h2⟩
-  repeat (split at h2 <;> simp at *); case _ h3 =>
-  · rcases h2 with ⟨h2, h4⟩
-    subst G'
+  intro h
+  fun_induction translate_SI generalizing G' <;> simp [pure, Except.pure] at *
+  case _ =>
+    subst h; constructor
+  case _ ctors _ ih =>
+    cases wf; case _ wftl wfhd =>
+    simp [bind, Except.bind_eq_ok_iff] at h; rcases h with ⟨Γ', h1, h⟩
+    split at h <;> simp at h
+    subst G'; case _ h =>
+    rcases h with ⟨h2, h⟩;
+    simp [Vec.all_eq_true] at h;
     cases wfhd; case _ c1 c2 c3 =>
     constructor
-    · apply Intermediate.GlobalWf.classDecl
-      apply h3
-      · { intro i j hi hj ne; replace c2 := c2 i j (by grind) (by grind) ne; grind }
-      · intro i mn R T tys hi tsp tys_shape; replace c3 := c3 i mn R (by grind);
-        simp; rcases c3 with ⟨c3a, c3b, c3c, c3d⟩;
-        apply And.intro
-        · { simp [c3a, mk_method_om]; rw[c3a]; simp; sorry }
-        · apply And.intro; apply c3b; sorry
+    · apply Intermediate.GlobalWf.data
+      · intro i y T h3; replace c3 := c3 i y T h3
+        apply And.intro; sorry; apply And.intro; apply c3.1; sorry
+      · apply c2
+      · apply h2
     · apply ih wftl h1
+  case _ ih => -- defn
+    cases wf; case _ wftl wfhd =>
+    simp [bind, Except.bind_eq_ok_iff] at h; rcases h with ⟨Γ', h1, h⟩
+    split at h <;> simp at h
+    case _ h2 =>
+      subst G'
+      cases wfhd
+      constructor
+      · apply Intermediate.GlobalWf.defn
+        sorry -- needs kind inference defined on Intermediate Global
+        apply h2
+      · apply ih wftl h1
 
-case _ ih => -- instance
-  simp [bind, Except.bind_eq_ok_iff] at h; rcases h with ⟨Γ', h1, h⟩
-  split at h <;> try simp [Except.bind] at h
-  split at h <;> try simp at h
-  split at h <;> try simp at h
-  split at h <;> try simp at h
-  split at h <;> try simp at h
-  split at h <;> try simp at h
-  subst G'
-  case _ h2 _ _ h3 _ _ _ _ h4 h5 _ mths h6 h7  =>
-  rcases h5 with ⟨e1, e2⟩; subst e1
-  cases wf; case _ cls_name _ K mτs _ wftl wfhd =>
-  cases wfhd; case _ _ _ _ _ _ _ rsp' _ _ _ lks _ q1 e _ =>
-  simp at q1; rcases q1 with ⟨e1, q1⟩; subst e1; simp at q1; rcases q1 with ⟨e1, q1⟩; subst e1
-  rcases q1 with ⟨e1, q1⟩; subst e1; simp at q1; rcases q1 with ⟨e1, q1⟩; subst e1;
-  rcases q1 with ⟨e1, q1⟩; subst e1; simp at q1; rcases q1 with ⟨e1, q1⟩; subst e1; subst q1
-  simp [Option.toTM] at cls_name; split at cls_name <;> simp at *; simp[Except.pure] at cls_name; cases cls_name
-  case _ h3 =>
-  rw[rsp'] at h3; cases h3; simp at h4
-  have lem := translate_SI_lookup_odata wftl h1 lks h4; rcases lem with ⟨e1, e2⟩; subst e1; subst e2
-  simp at h4 h6
-  constructor
-  · apply Intermediate.GlobalWf.inst
-    assumption
-    apply h4
-    apply h7
-    · intro i hi;
-      have lem := mk_inst_mths_SI_sound h6
-      have lem2 := mk_inst_mths_SI_indexing h6 i hi
-      rcases lem2 with ⟨j, h, lem2, lem3⟩
-      exists j; exists h; apply And.intro
-      symm; assumption
-      replace lem := lem mths[j] (by simp); simp at lem
-      rcases lem with ⟨mn, n, na, nb, v, t, lem⟩; rw[lem]; simp
-      rw[lem] at lem3; simp at lem3; symm; assumption
-  · apply ih wftl h1
+  case _ kc s Ks mτs Γ ih =>  -- class decl
+    cases wf; case _ wftl wfhd =>
+    simp [bind, Except.bind_eq_ok_iff] at h; rcases h with ⟨Γ', h1, h2⟩
+    repeat (split at h2 <;> simp at *); case _ h3 =>
+    · rcases h2 with ⟨h2, h4⟩
+      subst G'
+      cases wfhd; case _ c1 c2 c3 =>
+      constructor
+      · apply Intermediate.GlobalWf.classDecl
+        apply h3
+        · { intro i j hi hj ne; replace c2 := c2 i j (by grind) (by grind) ne; grind }
+        · intro i mn R T tys hi tsp tys_shape; replace c3 := c3 i mn R (by grind);
+          simp; rcases c3 with ⟨c3a, c3b, c3c, c3d⟩;
+          apply And.intro
+          · { simp [c3a, mk_method_om]; rw[c3a]; simp; sorry }
+          · apply And.intro; apply c3b; sorry
+      · apply ih wftl h1
+
+  case _ ih => -- instance
+    simp [bind, Except.bind_eq_ok_iff] at h; rcases h with ⟨Γ', h1, h⟩
+    split at h <;> try simp [Except.bind] at h
+    split at h <;> try simp at h
+    split at h <;> try simp at h
+    split at h <;> try simp at h
+    split at h <;> try simp at h
+    split at h <;> try simp at h
+    subst G'
+    case _ h2 _ _ h3 _ _ _ _ h4 h5 _ mths h6 h7  =>
+    rcases h5 with ⟨e1, e2⟩; subst e1
+    cases wf; case _ cls_name _ K mτs _ wftl wfhd =>
+    cases wfhd; case _ _ _ _ _ _ _ rsp' _ _ _ lks _ q1 e _ =>
+    simp at q1; rcases q1 with ⟨e1, q1⟩; subst e1; simp at q1; rcases q1 with ⟨e1, q1⟩; subst e1
+    rcases q1 with ⟨e1, q1⟩; subst e1; simp at q1; rcases q1 with ⟨e1, q1⟩; subst e1;
+    rcases q1 with ⟨e1, q1⟩; subst e1; simp at q1; rcases q1 with ⟨e1, q1⟩; subst e1; subst q1
+    simp [Option.toTM] at cls_name; split at cls_name <;> simp at *; simp[Except.pure] at cls_name; cases cls_name
+    case _ h3 =>
+    rw[rsp'] at h3; cases h3; simp at h4
+    have lem := translate_SI_lookup_odata wftl h1 lks h4; rcases lem with ⟨e1, e2⟩; subst e1; subst e2
+    simp at h4 h6
+    constructor
+    · apply Intermediate.GlobalWf.inst
+      assumption
+      apply h4
+      apply h7
+      · intro i hi;
+        have lem := mk_inst_mths_SI_sound h6
+        have lem2 := mk_inst_mths_SI_indexing h6 i hi
+        rcases lem2 with ⟨j, h, lem2, lem3⟩
+        exists j; exists h; apply And.intro
+        symm; assumption
+        replace lem := lem mths[j] (by simp);
+        rcases lem with ⟨mn, n, na, nb, v, t, lem⟩; rw[lem]; simp
+        rw[lem] at lem3; simp at lem3; symm; assumption
+    · apply ih wftl h1
 
 
 
@@ -459,22 +475,22 @@ theorem Intermediate.Query.strength_inst1 {Γ : Intermediate.GlobalEnv} :
   T.spine = some (cls2, tys) ->
   q ≠ iname ->
   Intermediate.Query Γ v #(q) #(T)
-  := by
-intro h1 h2 h3
-cases h1; case _ h1 h4 =>
-simp [Intermediate.lookup_ctor?, h2, Intermediate.lookup_ctor?, Intermediate.lookup] at h1;
-constructor
-have lem : (q = iname) = False := by grind;
-generalize ite_def : (if q = iname then
-            some
-              (Intermediate.Entry.octor iname
-                ⟨na, (KsU, ⟨nb, (KsE, ⟨nc, (Tys, (gt#cls1).mkApps_nats (List.range na).reverse)⟩)⟩)⟩)
-          else Intermediate.lookup q Γ) = ite at *
-conv at ite_def =>
-  lhs
-  simp [ite_cond_eq_false (h := by apply lem)]
-simp [Intermediate.lookup_ctor?, h2, ite_def]; apply h1
-constructor
+:= by
+  intro h1 h2 h3
+  cases h1; case _ h1 h4 =>
+  simp [Intermediate.lookup_ctor?, h2, Intermediate.lookup_ctor?, Intermediate.lookup] at h1;
+  constructor
+  have lem : (q = iname) = False := by grind;
+  generalize ite_def : (if q = iname then
+              some
+                (Intermediate.Entry.octor iname
+                  ⟨na, (KsU, ⟨nb, (KsE, ⟨nc, (Tys, (gt#cls1).mkApps_nats (List.range na).reverse)⟩)⟩)⟩)
+            else Intermediate.lookup q Γ) = ite at *
+  conv at ite_def =>
+    lhs
+    simp [ite_cond_eq_false (h := by apply lem)]
+  simp [Intermediate.lookup_ctor?, h2, ite_def]; apply h1
+  constructor
 
 
 
@@ -482,48 +498,48 @@ theorem Intermediate.lookup_openm_shape {G : Intermediate.GlobalEnv} (wf : ⊢ G
   Intermediate.lookup mn G = some (Intermediate.Entry.openm mn cls spTy) ->
   ∃ na Ks1 T R tys, spTy = ⟨na, Ks1, 0, #(), 1, #(T), R⟩ ∧ T.spine = some (cls, tys)
 := by
-intro h
-induction wf
-case _ => simp [Intermediate.lookup] at h
-case _ wfhd wftl ih =>
-  cases wfhd
-  case data =>
-    simp [Intermediate.lookup] at h; split at h
-    case _ e => subst e; simp at h
-    case _ =>
-      replace h := Vec.fold_or h
-      cases h
-      case _ h => apply ih h
-      case _ h => rcases h with ⟨i, h⟩; simp at h
-  case defn =>
-    simp [Intermediate.lookup] at h; split at h
-    case _ e => subst e; simp at h
-    case _ => apply ih h
-  case classDecl _ s mτs na Ks1 c1 c2 c3 =>
-    simp [Intermediate.lookup] at h; split at h
-    case _ e => subst e; simp at h
-    split at h
-    apply ih h
-    case _  h1 =>
-      simp [List.findIdx?_eq_some_iff_getElem] at h1
-      split at h;
-      · simp at h; rcases h with ⟨e1, e2, e3⟩; subst e1; subst e2; subst e3;
-        case _ i _ mn spTy h2 _ =>
-        rcases spTy with ⟨na', Ks1', nb', Ks2', nc', As', R⟩
-        simp [List.getElem?_eq_some_iff] at h2; rcases h2 with ⟨hi, h2⟩
-        let T := (Core.Ty.mkApps_nats (gt#s) ((List.range na)))
-        let tys := ((List.range na).map (t#·)).reverse
-        replace c3 := c3 i mn R T tys hi (by simp[T, tys, Core.Ty.mkApps_nats_spine]) rfl;
-        rcases c3 with ⟨c3a, c3b, c3c, c3d⟩
-        rw[h2] at c3a; cases c3a; simp
-        rcases h1 with ⟨h1, h2, h3⟩; subst h2; simp at *
-        exists na; exists Ks1; exists T; simp; exists tys
-        simp [T, tys, Core.Ty.mkApps_nats_spine]
-      · apply ih h
-  case inst =>
-    simp [Intermediate.lookup] at h; split at h
-    case _ e => subst e; simp at h
-    case _ => apply ih h
+  intro h
+  induction wf
+  case _ => simp [Intermediate.lookup] at h
+  case _ wfhd wftl ih =>
+    cases wfhd
+    case data =>
+      simp [Intermediate.lookup] at h; split at h
+      case _ e => subst e; simp at h
+      case _ =>
+        replace h := Vec.fold_or h
+        cases h
+        case _ h => apply ih h
+        case _ h => rcases h with ⟨i, h⟩; simp at h
+    case defn =>
+      simp [Intermediate.lookup] at h; split at h
+      case _ e => subst e; simp at h
+      case _ => apply ih h
+    case classDecl _ s mτs na Ks1 c1 c2 c3 =>
+      simp [Intermediate.lookup] at h; split at h
+      case _ e => subst e; simp at h
+      split at h
+      apply ih h
+      case _  h1 =>
+        simp [List.findIdx?_eq_some_iff_getElem] at h1
+        split at h;
+        · simp at h; rcases h with ⟨e1, e2, e3⟩; subst e1; subst e2; subst e3;
+          case _ i _ mn spTy h2 _ =>
+          rcases spTy with ⟨na', Ks1', nb', Ks2', nc', As', R⟩
+          simp [List.getElem?_eq_some_iff] at h2; rcases h2 with ⟨hi, h2⟩
+          let T := (Core.Ty.mkApps_nats (gt#s) ((List.range na)))
+          let tys := ((List.range na).map (t#·)).reverse
+          replace c3 := c3 i mn R T tys hi (by simp[T, tys, Core.Ty.mkApps_nats_spine]) rfl;
+          rcases c3 with ⟨c3a, c3b, c3c, c3d⟩
+          rw[h2] at c3a; cases c3a; simp
+          rcases h1 with ⟨h1, h2, h3⟩; subst h2; simp at *
+          exists na; exists Ks1; exists T; simp; exists tys
+          simp [T, tys, Core.Ty.mkApps_nats_spine]
+        · apply ih h
+    case inst =>
+      simp [Intermediate.lookup] at h; split at h
+      case _ e => subst e; simp at h
+      case _ => apply ih h
 
 theorem Intermediate.lookup_openm_index {G : Intermediate.GlobalEnv} (wf : ⊢ G):
   Intermediate.lookup mn G = some (Intermediate.Entry.openm mn cls spTy) ->
@@ -566,214 +582,217 @@ theorem Intermediate.lookup_none_ctor? :
 set_option maxHeartbeats 7000000
 theorem translate_SI_sound {G : Surface.GlobalEnv} {G' : Intermediate.GlobalEnv} (wf : ⊢ G) :
   ⟦ G ⟧ = .ok G' ->
-  Ω G' := by
-intro h
-have wf' := translate_SI_wf_sound wf h
-intro mn na nb nc Ks1 Ks2 Ts R qs _ h1 h2
-fun_induction translate_SI generalizing G' mn <;> simp [pure, Except.pure] at *
-· subst h; simp [Intermediate.lookup] at h1
-case _ ih => -- data
-  cases wf; case _ wftl wfhd =>
-  simp [bind, Except.bind_eq_ok_iff] at h; rcases h with ⟨Γ', h3, h⟩
-  split at h <;> simp at *
-  subst G'
-  cases wf'; case _ wftl' wfhd' =>
-  simp [Intermediate.lookup] at h1;
-  split at h1
-  case _ e => subst e; simp at h1
-  case _ e =>
-    replace h1 := Vec.fold_or h1
-    cases h1
-    case _ h1 =>
-      replace h2 := Intermediate.Query.opn_strengthen_ctor (by constructor; apply wfhd'; apply wftl') h2
-      replace ih := @ih _ wftl h3 wftl' mn h1 h2
-      rcases ih with ⟨i, n, cls, k1, k2, k3, Ks1, Ks2, tys, fds, scs, mths, ih⟩
-      exists i + 1; exists n; exists cls; exists k1; exists k2; exists k3;
-      exists Ks1; exists Ks2;
-      exists tys; exists fds
-      exists scs; exists mths
-    case _ h1 => rcases h1 with ⟨i, h1⟩; simp at h1
-case _ ih => -- defn decl
-  simp [bind, Except.bind_eq_ok_iff] at h; rcases h with ⟨Γ', h3, h⟩
-  split at h <;> simp at *
-  subst G'
-  cases wf; case _ wftl wfhd =>
-  cases wf'; case _ wftl' wfhd' =>
-  simp [Intermediate.lookup] at h1;
-  split at h1 <;> try simp at h1
-  replace h2 := Intermediate.Query.opn_strengthen_defn (by constructor; apply wfhd'; apply wftl') h2
-  replace ih := ih wftl h3 wftl' h1 h2
-  rcases ih with ⟨i, n, cls, k1, k2, k3, Ks1, Ks2, tys, fds, scs, mths, ih⟩
-  exists i + 1; exists n; exists cls; exists k1; exists k2; exists k3; exists Ks1; exists Ks2; exists tys; exists fds
-  exists scs; exists mths
-case _ cls _ _ _ mτs _ ih => -- class Decl
-  simp [bind, Except.bind_eq_ok_iff] at h; rcases h with ⟨Γ', h3, h⟩
-  split at h <;> simp at *
-  rcases h with ⟨h, h4⟩
-  subst G'
-  replace h2 := Intermediate.Query.opn_strengthen_class wf' h2
-  cases wf; case _ kc s _ _ _ wftl wfhd =>
-  cases wf'; case _ wftl' wfhd' =>
-  cases wfhd'; case _ ci1 ci2 ci3 =>
-  cases wfhd; case _ cs1 cs2 cs3 =>
-  simp [Intermediate.lookup] at h1
-  split at h1 <;> simp at *
-  split at h1 <;> simp at *
-  replace ih := ih wftl h3 wftl' h1 h2
-  rcases ih with ⟨i, n, cls, k1, k2, k3, Ks1, Ks2, tys, fds, scs, mths, ih⟩
-  exists i + 1; exists n; exists cls; exists k1; exists k2; exists k3; exists Ks1; exists Ks2;
-  exists tys; exists fds
-  exists scs; exists mths
-  split at h1 <;> simp at *
-  · case _ i _ _ cls _ e =>
-    rcases h1 with ⟨e1, e2, e3⟩; subst e1; subst e2; subst e3;
-    rcases e with ⟨mn', spty, e3, e4, e5⟩; subst e4; simp_all;
-    case _ lk =>
-    simp [List.findIdx?_eq_some_iff_getElem] at lk;
-    rcases lk with ⟨j, hj, lk⟩; subst hj;
-    simp [List.getElem?_eq_some_iff] at e3; rcases e3 with ⟨hi, e3⟩
-    rcases spty with ⟨na, Ks1, nb, Ks2, nc, As, R⟩
-    replace cs3 := cs3 i (mτs[i].fst) R hi
-    let T := (Core.Ty.mkApps_nats (gt#s) ((List.range kc)))
-    let tys := ((List.range kc).map (t#·)).reverse
-    replace ci3 := ci3 i (mτs[i].fst) R T tys hi (by simp[T, tys, Core.Ty.mkApps_nats_spine]) (by simp [tys])
-    rcases ci3 with ⟨ci3, ci4, ci5, ci6⟩; simp at ci3;
-    rcases cs3 with ⟨cs3, cs4, cs5, cs6⟩
-    unfold mk_method_om at ci3; rw [cs3] at ci3; simp at ci3;
-    unfold mk_method_om at e5; cases e5;
-    rw[cs3] at e3; cases e3
-    cases qs; case _ q qs =>
-    cases qs; simp at h2; cases h2; case _ h2 _ =>
-    simp [Intermediate.lookup_ctor?, Core.Ty.mkApps_nats_spine] at h2;
-    simp [Option.getD_eq_iff] at h2;
-    rcases h2 with ⟨ent, h2, h4⟩;  -- This will be ill typed
-    exfalso; apply Intermediate.lookup_none_ctor? ci1 h2 h4
-
-  · simp_all; replace ih := ih h1;
+  Ω G'
+:= by
+  intro h
+  have wf' := translate_SI_wf_sound wf h
+  intro mn na nb nc Ks1 Ks2 Ts R qs _ h1 h2
+  fun_induction translate_SI generalizing G' mn <;> simp [pure, Except.pure] at *
+  · subst h; simp [Intermediate.lookup] at h1
+  case _ ih => -- data
+    cases wf; case _ wftl wfhd =>
+    simp [bind, Except.bind_eq_ok_iff] at h; rcases h with ⟨Γ', h3, h⟩
+    split at h <;> simp at *
+    subst G'
+    cases wf'; case _ wftl' wfhd' =>
+    simp [Intermediate.lookup] at h1;
+    split at h1
+    case _ e => subst e; simp at h1
+    case _ e =>
+      replace h1 := Vec.fold_or h1
+      cases h1
+      case _ h1 =>
+        replace h2 := Intermediate.Query.opn_strengthen_ctor (by constructor; apply wfhd'; apply wftl') h2
+        replace ih := @ih _ wftl h3 wftl' mn h1 h2
+        rcases ih with ⟨i, n, cls, k1, k2, k3, Ks1, Ks2, tys, fds, scs, mths, ih⟩
+        exists i + 1; exists n; exists cls; exists k1; exists k2; exists k3;
+        exists Ks1; exists Ks2;
+        exists tys; exists fds
+        exists scs; exists mths
+      case _ h1 => rcases h1 with ⟨i, h1⟩; simp at h1
+  case _ ih => -- defn decl
+    simp [bind, Except.bind_eq_ok_iff] at h; rcases h with ⟨Γ', h3, h⟩
+    split at h <;> simp at *
+    subst G'
+    cases wf; case _ wftl wfhd =>
+    cases wf'; case _ wftl' wfhd' =>
+    simp [Intermediate.lookup] at h1;
+    split at h1 <;> try simp at h1
+    replace h2 := Intermediate.Query.opn_strengthen_defn (by constructor; apply wfhd'; apply wftl') h2
+    replace ih := ih wftl h3 wftl' h1 h2
+    rcases ih with ⟨i, n, cls, k1, k2, k3, Ks1, Ks2, tys, fds, scs, mths, ih⟩
+    exists i + 1; exists n; exists cls; exists k1; exists k2; exists k3; exists Ks1; exists Ks2; exists tys; exists fds
+    exists scs; exists mths
+  case _ cls _ _ _ mτs _ ih => -- class Decl
+    simp [bind, Except.bind_eq_ok_iff] at h; rcases h with ⟨Γ', h3, h⟩
+    split at h <;> simp at *
+    rcases h with ⟨h, h4⟩
+    subst G'
+    replace h2 := Intermediate.Query.opn_strengthen_class wf' h2
+    cases wf; case _ kc s _ _ _ wftl wfhd =>
+    cases wf'; case _ wftl' wfhd' =>
+    cases wfhd'; case _ ci1 ci2 ci3 =>
+    cases wfhd; case _ cs1 cs2 cs3 =>
+    simp [Intermediate.lookup] at h1
+    split at h1 <;> simp at *
+    split at h1 <;> simp at *
+    replace ih := ih wftl h3 wftl' h1 h2
     rcases ih with ⟨i, n, cls, k1, k2, k3, Ks1, Ks2, tys, fds, scs, mths, ih⟩
     exists i + 1; exists n; exists cls; exists k1; exists k2; exists k3; exists Ks1; exists Ks2;
     exists tys; exists fds
     exists scs; exists mths
-
-case _ cls1 iname na Ks1 nb Ks2 nc As R _ _ ih =>
-  cases wf; case _ wftl wfhd =>
-  cases wfhd; case _ cls2 _ _ _ _ _ _ _ _ _ _ _ _ _ _ _ _ lks _ q1 q2 q3 =>
-  simp [bind, Except.bind_eq_ok_iff] at h; rcases h with ⟨Γ', h, h3⟩
-  split at h3
-  · simp [Option.toTM] at h3
-    · split at h3 <;> simp [Except.bind] at h3
-      repeat (split at h3 <;> try simp at h3)
-      subst G';
-      cases wf'; case _ wftl' wfhd' =>
-      cases wfhd'; case _ rsp _ _ _ _ _ _ _ _ rsp' _ _ e _ _ _ _ _ lki1 e1 _ v mths_comp _ _ _ _ _ lki2 _ _ =>
-      cases e; rcases e1 with ⟨e1, e2⟩; cases e1
-      simp at q1; rcases q1 with ⟨e1, q1⟩; subst e1; simp at q1; rcases q1 with ⟨e1, q1⟩; subst e1
-      rcases q1 with ⟨e1, q1⟩; subst e1; simp at q1; rcases q1 with ⟨e1, q1⟩; subst e1;
-      rcases q1 with ⟨e1, q1⟩; subst e1; simp at q1; rcases q1 with ⟨e1, q1⟩; subst e1; subst q1
-      rw[rsp] at rsp'; simp at rsp'; rcases rsp' with ⟨e1, e2⟩; rw[lki1] at lki2; cases lki2
-      simp at lki1; simp at *;
-      simp [Intermediate.lookup] at h1
-      split at h1
-      simp at h1
-      have e := translate_SI_lookup_odata wftl h lks lki1
-      rcases e with ⟨e1, e2⟩; subst e1; subst e2;
-      have lem := Intermediate.lookup_openm_shape wftl' h1
-      rcases lem with ⟨na, Ks1, T, R, tys, e⟩
-      simp at e; rcases e with ⟨⟨e1, e2⟩, e3⟩; subst e1; simp at e2; rcases e2 with ⟨e2a, e2b, e2⟩;
-      subst e2a; subst e2b; simp at e2; rcases e2 with ⟨e2a, e2b, e2⟩; subst e2a; subst e2b; simp at e2;
-      rcases e2 with ⟨e2a, e2b⟩; subst e2a; subst e2b;
+    split at h1 <;> simp at *
+    · case _ i _ _ cls _ e =>
+      rcases h1 with ⟨e1, e2, e3⟩; subst e1; subst e2; subst e3;
+      rcases e with ⟨mn', spty, e3, e4, e5⟩; subst e4; simp_all;
+      case _ lk =>
+      simp [List.findIdx?_eq_some_iff_getElem] at lk;
+      rcases lk with ⟨j, hj, lk⟩; subst hj;
+      simp [List.getElem?_eq_some_iff] at e3; rcases e3 with ⟨hi, e3⟩
+      rcases spty with ⟨na, Ks1, nb, Ks2, nc, As, R⟩
+      replace cs3 := cs3 i (mτs[i].fst) R hi
+      let T := (Core.Ty.mkApps_nats (gt#s) ((List.range kc)))
+      let tys := ((List.range kc).map (t#·)).reverse
+      replace ci3 := ci3 i (mτs[i].fst) R T tys hi (by simp[T, tys, Core.Ty.mkApps_nats_spine]) (by simp [tys])
+      rcases ci3 with ⟨ci3, ci4, ci5, ci6⟩; simp at ci3;
+      rcases cs3 with ⟨cs3, cs4, cs5, cs6⟩
+      unfold mk_method_om at ci3; rw [cs3] at ci3; simp at ci3;
+      unfold mk_method_om at e5; cases e5;
+      rw[cs3] at e3; cases e3
       cases qs; case _ q qs =>
-      cases qs
-      cases decEq q iname
-      case _ e =>
-        -- q ≠ iname
-        cases decEq cls1 cls2
-        case _ e' =>
-          replace e' : cls2 ≠ cls1 := by grind
-          replace e : q ≠ iname := by grind
-          have lem1 := Intermediate.Query.strength_inst1 h2 e3 e
-          replace ih := ih wftl h wftl' h1 lem1
-          rcases ih with ⟨i, n, cls_name, k1, k2, k3, Ks1, Ks2, As, fds, scs, mths, ih⟩
-          exists i + 1; exists n; exists cls_name; exists k1; exists k2; exists k3; exists Ks1; exists Ks2
-          exists As; exists fds; exists scs; exists mths
-        case _ e' => -- cls = cls2
-          subst e'
-          replace e : q ≠ iname := by grind
-          have lem1 := Intermediate.Query.strength_inst1 h2 e3 e
-          replace ih := ih wftl h wftl' h1 lem1
-          rcases ih with ⟨i, n, cls_name, k1, k2, k3, Ks1, Ks2, As, fds, scs, mths, ih⟩
-          exists i + 1; exists n; exists cls_name; exists k1; exists k2; exists k3; exists Ks1; exists Ks2
-          exists As; exists fds; exists scs; exists mths
-      case _ e => -- q = iname
-        subst e
-        cases decEq cls1 cls2
-        case _ e => -- cls1 ≠ cls2
-          exfalso
-          cases h2; case _ h1 h2 =>
-          simp [Intermediate.lookup_ctor?] at h1; rw[e3] at h1; split at h1 <;> simp at *
-          simp [Intermediate.lookup, Intermediate.Entry.ctor?] at h1;
-          have lem := Core.Ty.mkApps_nats_spine cls2 (List.range na).reverse
-          simp [lem] at h1; case _ e' => rcases e' with ⟨e'', e'⟩; subst e''; apply e; symm; apply h1
+      cases qs; simp at h2; cases h2; case _ h2 _ =>
+      simp [Intermediate.lookup_ctor?, Core.Ty.mkApps_nats_spine] at h2;
+      simp [Option.getD_eq_iff] at h2;
+      rcases h2 with ⟨ent, h2, h4⟩;  -- This will be ill typed
+      exfalso; apply Intermediate.lookup_none_ctor? ci1 h2 h4
+
+    · simp_all; replace ih := ih h1;
+      rcases ih with ⟨i, n, cls, k1, k2, k3, Ks1, Ks2, tys, fds, scs, mths, ih⟩
+      exists i + 1; exists n; exists cls; exists k1; exists k2; exists k3; exists Ks1; exists Ks2;
+      exists tys; exists fds
+      exists scs; exists mths
+
+  case _ cls1 iname na Ks1 nb Ks2 nc As R _ _ ih =>
+    cases wf; case _ wftl wfhd =>
+    cases wfhd; case _ cls2 _ _ _ _ _ _ _ _ _ _ _ _ _ _ _ _ lks _ q1 q2 q3 =>
+    simp [bind, Except.bind_eq_ok_iff] at h; rcases h with ⟨Γ', h, h3⟩
+    split at h3
+    · simp [Option.toTM] at h3
+      · split at h3 <;> simp [Except.bind] at h3
+        repeat (split at h3 <;> try simp at h3)
+        subst G';
+        cases wf'; case _ wftl' wfhd' =>
+        cases wfhd'; case _ rsp _ _ _ _ _ _ _ _ rsp' _ _ e _ _ _ _ _ lki1 e1 _ v mths_comp _ _ _ _ _ lki2 _ _ =>
+        cases e; rcases e1 with ⟨e1, e2⟩; cases e1
+        simp at q1; rcases q1 with ⟨e1, q1⟩; subst e1; simp at q1; rcases q1 with ⟨e1, q1⟩; subst e1
+        rcases q1 with ⟨e1, q1⟩; subst e1; simp at q1; rcases q1 with ⟨e1, q1⟩; subst e1;
+        rcases q1 with ⟨e1, q1⟩; subst e1; simp at q1; rcases q1 with ⟨e1, q1⟩; subst e1; subst q1
+        rw[rsp] at rsp'; simp at rsp'; rcases rsp' with ⟨e1, e2⟩; rw[lki1] at lki2; cases lki2
+        simp at lki1; simp at *;
+        simp [Intermediate.lookup] at h1
+        split at h1
+        simp at h1
+        have e := translate_SI_lookup_odata wftl h lks lki1
+        rcases e with ⟨e1, e2⟩; subst e1; subst e2;
+        have lem := Intermediate.lookup_openm_shape wftl' h1
+        rcases lem with ⟨na, Ks1, T, R, tys, e⟩
+        simp at e; rcases e with ⟨⟨e1, e2⟩, e3⟩; subst e1; simp at e2; rcases e2 with ⟨e2a, e2b, e2⟩;
+        subst e2a; subst e2b; simp at e2; rcases e2 with ⟨e2a, e2b, e2⟩; subst e2a; subst e2b; simp at e2;
+        rcases e2 with ⟨e2a, e2b⟩; subst e2a; subst e2b;
+        cases qs; case _ q qs =>
+        cases qs
+        cases decEq q iname
         case _ e =>
+          -- q ≠ iname
+          cases decEq cls1 cls2
+          case _ e' =>
+            replace e' : cls2 ≠ cls1 := by grind
+            replace e : q ≠ iname := by grind
+            have lem1 := Intermediate.Query.strength_inst1 h2 e3 e
+            replace ih := ih wftl h wftl' h1 lem1
+            rcases ih with ⟨i, n, cls_name, k1, k2, k3, Ks1, Ks2, As, fds, scs, mths, ih⟩
+            exists i + 1; exists n; exists cls_name; exists k1; exists k2; exists k3; exists Ks1; exists Ks2
+            exists As; exists fds; exists scs; exists mths
+          case _ e' => -- cls = cls2
+            subst e'
+            replace e : q ≠ iname := by grind
+            have lem1 := Intermediate.Query.strength_inst1 h2 e3 e
+            replace ih := ih wftl h wftl' h1 lem1
+            rcases ih with ⟨i, n, cls_name, k1, k2, k3, Ks1, Ks2, As, fds, scs, mths, ih⟩
+            exists i + 1; exists n; exists cls_name; exists k1; exists k2; exists k3; exists Ks1; exists Ks2
+            exists As; exists fds; exists scs; exists mths
+        case _ e => -- q = iname
           subst e
-          exists 0; exists q; exists cls1; exists na; exists nb; exists nc; exists Ks1; exists Ks2;
-          exists As; exists []; exists []; exists v; simp
-          have lem := mk_inst_mths_SI_sound mths_comp
-          have lem1 := mk_inst_mths_SI_indexing mths_comp
-          have lem2 := Intermediate.lookup_openm_index wftl' h1 lki1
-          rcases lem2 with ⟨j, hj, lem2⟩; subst lem2
-          replace lem1 := lem1 j hj
-          rcases lem1 with ⟨i, hi, lem1a, lem2a⟩
-          replace lem := lem v[i] (by grind)
-          rcases lem with ⟨mn', n, na, nb, v', t, lem⟩
-          exists i; exists (v[i]).2.2.2; rw[lem]; simp
-          exists #((q, ⟨n, (v', na, nb)⟩));
-          apply And.intro
-          grind
-          constructor; grind; simp; constructor
-  · simp at h3
+          cases decEq cls1 cls2
+          case _ e => -- cls1 ≠ cls2
+            exfalso
+            cases h2; case _ h1 h2 =>
+            simp [Intermediate.lookup_ctor?] at h1; rw[e3] at h1; split at h1 <;> simp at *
+            simp [Intermediate.lookup, Intermediate.Entry.ctor?] at h1;
+            have lem := Core.Ty.mkApps_nats_spine cls2 (List.range na).reverse
+            simp [lem] at h1; case _ e' => rcases e' with ⟨e'', e'⟩; subst e''; apply e; symm; apply h1
+          case _ e =>
+            subst e
+            exists 0; exists q; exists cls1; exists na; exists nb; exists nc; exists Ks1; exists Ks2;
+            exists As; exists []; exists []; exists v; simp
+            have lem := mk_inst_mths_SI_sound mths_comp
+            have lem1 := mk_inst_mths_SI_indexing mths_comp
+            have lem2 := Intermediate.lookup_openm_index wftl' h1 lki1
+            rcases lem2 with ⟨j, hj, lem2⟩; subst lem2
+            replace lem1 := lem1 j hj
+            rcases lem1 with ⟨i, hi, lem1a, lem2a⟩
+            replace lem := lem v[i] (by grind)
+            rcases lem with ⟨mn', n, na, nb, v', t, lem⟩
+            exists i; exists (v[i]).2.2.2; rw[lem]; simp
+            exists #((q, ⟨n, (v', na, nb)⟩));
+            apply And.intro
+            grind
+            constructor; grind; simp; constructor
+    · simp at h3
 
 
 theorem translate_IC_query {G : Intermediate.GlobalEnv} {G' : Core.GlobalEnv} (wf : ⊢ G):
   ⟦ G ⟧ = Except.ok G' ->
   Core.Query G' Core.DataConst.opn q Ts ->
-  Intermediate.Query G Intermediate.DataConst.opn q Ts := by
-intro h1 h2
-simp at h1 h2
-induction h2
-case nil  => constructor
-case cons h _ ih =>
-  constructor
-  simp [Core.lookup_ctor?] at h;
-  split at h;
-  · simp [Option.getD_eq_iff] at h;
-    rcases h with ⟨ent, lk, h⟩
-    cases ent <;> simp [Core.Entry.ctor?] at h
+  Intermediate.Query G Intermediate.DataConst.opn q Ts
+:= by
+  intro h1 h2
+  simp at h1 h2
+  induction h2
+  case nil  => constructor
+  case cons h _ ih =>
+    constructor
+    simp [Core.lookup_ctor?] at h;
     split at h;
-    simp at h; subst h; case _ oc R _ _ _ e1 e2 =>
-      simp [Intermediate.lookup_ctor?]; rw[e2]; simp; simp [Option.getD_eq_iff];
-      exists Intermediate.Entry.octor oc R
-      apply And.intro
-      case _ => apply translate_IC_lookup_some_octor wf h1 lk
-      simp [Intermediate.Entry.ctor?, e1]
-    cases h
-  · cases h
-  apply ih
+    · simp [Option.getD_eq_iff] at h;
+      rcases h with ⟨ent, lk, h⟩
+      cases ent <;> simp [Core.Entry.ctor?] at h
+      split at h;
+      simp at h; subst h; case _ oc R _ _ _ e1 e2 =>
+        simp [Intermediate.lookup_ctor?]; rw[e2]; simp; simp [Option.getD_eq_iff];
+        exists Intermediate.Entry.octor oc R
+        apply And.intro
+        case _ => apply translate_IC_lookup_some_octor wf h1 lk
+        simp [Intermediate.Entry.ctor?, e1]
+      cases h
+    · cases h
+    apply ih
 
 
 theorem mk_inst_mth_IC_shape :
   mk_inst_mth_IC Γ' mn m p t = Except.ok i ->
-  ∃ b, i = .inst mn p b := by
-intro h
-unfold mk_inst_mth_IC at h
-split at h <;> simp at *
-split at h <;> simp [bind] at *
-case _ e =>
-  rcases e with ⟨e1, e2⟩; subst e1; subst e2
-  simp [Except.bind_eq_ok_iff] at h; rcases h with ⟨Δ, Γ, h⟩
-  simp [Functor.map, Except.map] at h; rcases h with ⟨_, h⟩
-  repeat (split at h <;> simp [Option.toTM] at *)
-  case _ v _ => symm at h; exists v
+  ∃ b, i = .inst mn p b
+:= by
+  intro h
+  unfold mk_inst_mth_IC at h
+  split at h <;> simp at *
+  split at h <;> simp [bind] at *
+  case _ e =>
+    rcases e with ⟨e1, e2⟩; subst e1; subst e2
+    simp [Except.bind_eq_ok_iff] at h; rcases h with ⟨Δ, Γ, h⟩
+    simp [Functor.map, Except.map] at h; rcases h with ⟨_, h⟩
+    repeat (split at h <;> simp [Option.toTM] at *)
+    case _ v _ => symm at h; exists v
 
 
 theorem mk_inst_mths_IC_lookup :
@@ -853,9 +872,9 @@ theorem translate_IC_indexing_inst_mths {G : Intermediate.GlobalEnv} {G' : Core.
     replace ih := ih wftl h3 h2
     rcases ih with ⟨i, b, p, ih1, ih2⟩;
     exists ((List.map (fun x => Core.Global.openm x.fst x.snd) mths).length + 1 + i); exists b; exists p
-
-    have lem := List.getElem?_append_right (l₁ := List.map (fun x => Core.Global.openm x.fst x.snd) mths ++ [Core.Global.odata s (mk_cls_kind K)]) (l₂ := Γ') (i := (List.map (fun x => Core.Global.openm x.fst x.snd) mths).length + 1 + i) (by grind)
-    simp at lem; grind
+    -- have lem := List.getElem?_append_right (l₁ := List.map (fun x => Core.Global.openm x.fst x.snd) mths ++ [Core.Global.odata s (mk_cls_kind K)]) (l₂ := Γ') (i := (List.map (fun x => Core.Global.openm x.fst x.snd) mths).length + 1 + i) (by grind)
+    -- simp at lem; grind
+    sorry
 
   case _ iname cls_name k1 k2 k3 Ks1 Ks2 tys _ _ _ _ ih => -- inst
     simp [bind, Except.bind_eq_ok_iff] at h1
@@ -873,7 +892,7 @@ theorem translate_IC_indexing_inst_mths {G : Intermediate.GlobalEnv} {G' : Core.
       subst e10; subst e11
       replace h3 := mk_inst_mths_indexing mths_comp h3
       rcases h3 with ⟨b, h3⟩;
-      exists j1; exists b; exists p; grind
+      exists j1; exists b; exists p; sorry -- grind
 
     case _ =>
       replace ih := ih wftl h1 h2
@@ -881,59 +900,89 @@ theorem translate_IC_indexing_inst_mths {G : Intermediate.GlobalEnv} {G' : Core.
       exists mths'.length + 1 + j1; exists b; exists p;
       grind
 
+theorem lookup_kind_IC_some {G : Intermediate.GlobalEnv} {G' : Core.GlobalEnv} (wf : ⊢ G) (h : ⟦ G ⟧ = .ok G') :
+  Intermediate.lookup_kind G x = some K -> Core.lookup_kind G' x = some K
+:= by
+  intro h1
+  unfold Intermediate.lookup_kind at h1
+  unfold Core.lookup_kind
+  generalize lki_def : Intermediate.lookup x G = lki at *
+  cases lki <;> simp at *
+  case _ v =>
+  cases v <;> simp [Intermediate.Entry.kind] at *
+  subst h1; sorry
+  sorry
+
+theorem kinding_transfer {G : Intermediate.GlobalEnv} {G' : Core.GlobalEnv} (wf : ⊢ G) (h : ⟦ G ⟧ = .ok G') :
+  G&Δ ⊢ T : K ->  G'&Δ ⊢ T : K
+| .var h1 => .var h1
+| .global h1 => .global (lookup_kind_IC_some wf h h1)
+| .app h1 h2 => .app (kinding_transfer wf h h1) (kinding_transfer wf h h2)
+| .arrow h1 h2 => .arrow (kinding_transfer wf h h1) (kinding_transfer wf h h2)
+| .all h1 => .all (kinding_transfer wf h h1)
+| .eq h1 h2 => .eq (kinding_transfer wf h h1) (kinding_transfer wf h h2)
+
 
 theorem translate_IC_lookup_none {G : Intermediate.GlobalEnv} {G' : Core.GlobalEnv} (wf : ⊢ G) :
   ⟦ G ⟧ = .ok G' ->
   Intermediate.lookup x G = none ->
   Core.lookup x G' = none := by sorry
 
-theorem translate_IC_spine_kinding {G : Intermediate.GlobalEnv} {G' : Core.GlobalEnv} (wf : ⊢ G) :
+theorem translate_IC_spine_kinding {G : Intermediate.GlobalEnv} {G' : Core.GlobalEnv} (wf : ⊢ G) (ht : ⟦G⟧ = Except.ok G') (lk : Intermediate.lookup s G = none) :
   Intermediate.SpineKinding (Intermediate.SpCtorVariant.data Intermediate.DataConst.cls) y (Intermediate.Global.data { name := s, kind := K, ctors := ⟨0, #()⟩ } :: G) (Core.Ty.is_data s) T ->
   Core.SpineKinding (Core.SpCtorVariant.data Core.DataConst.cls) y (Core.Global.data 0 s K #() :: G') (Core.Ty.is_data s) T
 := by
-intro h
-cases h; case _ m1 m2 n Δ R Ks1 Ks2 Ts h1 h2 h3 h4 h5 =>
-constructor
-apply h1
-sorry -- transfer lemmas for well kindedness
-sorry
-apply h4
-intro e i; simp at e
-
-
+  intro h
+  cases h; case _ m1 m2 n Δ R Ks1 Ks2 Ts h1 h2 h3 h4 h5 =>
+  constructor
+  apply h1
+  intro i; replace h2 := h2 i;
+  apply kinding_transfer (G' := (Core.Global.data 0 s K #() :: G'))
+    (by constructor; constructor; simp; simp; apply lk; apply wf)
+    (by simp [translate_IC, Functor.map, Except.map_eq_ok_iff, ht]) h2; -- transfer lemmas for well kindedness
+  apply kinding_transfer (G' := (Core.Global.data 0 s K #() :: G'))
+    (by constructor; constructor; simp; simp; apply lk; apply wf)
+    (by simp [translate_IC, Functor.map, Except.map_eq_ok_iff, ht])
+    h3
+  apply h4
+  intro e i; simp at e
 
 
 theorem translate_IC_wf_sound {G : Intermediate.GlobalEnv} {G' : Core.GlobalEnv} (wf : ⊢ G):
   ⟦ G ⟧ = .ok G' ->
   ⊢ G'
 := by
-intro h
-fun_induction translate_IC generalizing G' <;> simp [pure, bind] at h
-case _ => -- nil
-  cases h; constructor
-case _ ih => -- data
-  simp [Except.bind_eq_ok_iff] at h; rcases h with ⟨Γ', h, h1⟩
-  cases h1
-  cases wf; case _ wftl wfhd =>
-  cases wfhd; case _ c1 c2 c3 =>
-  apply Core.ListGlobalWf.cons
-  apply Core.GlobalWf.data
-  intro i y T e; replace c3 := c3 i y T e; rcases c3 with ⟨c1, c2, c3⟩;
-  apply And.intro; apply translate_IC_spine_kinding wftl c1; apply And.intro; apply c2; apply translate_IC_lookup_none wftl h c3
-  apply c2
-  apply translate_IC_lookup_none wftl h c1
-  apply ih wftl h
-case _ ih => -- defn
-  sorry
-case _ ih => -- class
-  sorry
-case _ fds scs mths _ ih => -- inst
-  simp [Except.bind_eq_ok_iff] at h; rcases h with ⟨Γ', h, h1, h2, h3⟩;
-  cases h3;
-  cases wf; case _ wftl wfhd =>
-  cases wfhd; case _ h1 h2 h3 h4 =>
-  replace ih := ih wftl h
-  sorry
+  intro h
+  fun_induction translate_IC generalizing G' <;> simp [pure, bind] at h
+  case _ => -- nil
+    cases h; constructor
+  case _ ih => -- data
+    simp [Except.bind_eq_ok_iff] at h; rcases h with ⟨Γ', h, h1⟩
+    cases h1
+    cases wf; case _ wftl wfhd =>
+    cases wfhd; case _ c1 c2 c3 =>
+    apply Core.ListGlobalWf.cons
+    apply Core.GlobalWf.data
+    intro i y T e; replace c3 := c3 i y T e; rcases c3 with ⟨c1', c2', c3'⟩;
+    apply And.intro; apply translate_IC_spine_kinding wftl h c1 c1'; apply And.intro; apply c2'; apply translate_IC_lookup_none wftl h c3'
+    apply c2
+    apply translate_IC_lookup_none wftl h c1
+    apply ih wftl h
+  case _ ih => -- defn
+    sorry
+  case _ ih => -- class
+    sorry
+  case _ iname cls_name k1 k2 k3 Ks1 Ks2 As fds scs mths _ ih => -- inst
+    simp [Except.bind_eq_ok_iff] at h; rcases h with ⟨Γ', h, h1, h2, h3⟩;
+    cases h3;
+    cases wf; case _ wftl wfhd =>
+    cases wfhd; case _ h1 h2 h3 h4 =>
+    replace ih := ih wftl h
+    have lem : Core.GlobalWf Γ' (.octor iname ⟨k1, Ks1, k2, Ks2, k3, (Vec.map (fun x => t#x.snd ~[★]~ x.fst) (As.zip (Vec.range k3)),
+                      (gt#cls_name).mkApps_nats (List.range k3).reverse)⟩) := by constructor; sorry; apply translate_IC_lookup_none wftl h h1
+    replace ih := Core.ListGlobalWf.cons lem ih
+
+    sorry
 
 
 
@@ -941,138 +990,140 @@ case _ fds scs mths _ ih => -- inst
 theorem translate_IC_lookup_openm {G : Intermediate.GlobalEnv} {G' : Core.GlobalEnv} (wf : ⊢ G) :
   ⟦ G ⟧ = .ok G' ->
   Core.lookup mn G' = some (Core.Entry.openm mn ⟨na, (Ks1, ⟨nb, (Ks2, ⟨nc, (Ts, R)⟩)⟩)⟩) ->
-  ∃ cls, Intermediate.lookup mn G = some (Intermediate.Entry.openm mn cls ⟨na, (Ks1, ⟨nb, (Ks2, ⟨nc, (Ts, R)⟩)⟩)⟩) := by
-intro h1 h2
-have wf' := translate_IC_wf_sound wf h1
-simp at h1 h2
-fun_induction translate_IC generalizing G' mn <;> simp at *
-case _ =>
-  simp [pure, Except.pure] at h1; subst h1; simp [Core.lookup] at h2
-case _ ih =>
-  cases wf; case _ wftl wfhd =>
-  cases wfhd;
-  simp [Functor.map, Except.map_eq_ok_iff] at h1;
-  rcases h1 with ⟨Γ', h1, h2⟩; subst G'
-  simp [Core.lookup] at h2; split at h2 <;> try simp at h2
-  replace h2 := Vec.fold_or h2
-  cases h2
-  case _ h2 =>
+  ∃ cls, Intermediate.lookup mn G = some (Intermediate.Entry.openm mn cls ⟨na, (Ks1, ⟨nb, (Ks2, ⟨nc, (Ts, R)⟩)⟩)⟩)
+:= by
+  intro h1 h2
+  have wf' := translate_IC_wf_sound wf h1
+  simp at h1 h2
+  fun_induction translate_IC generalizing G' mn <;> try simp at *
+  case _ =>
+    simp [pure, Except.pure] at h1; subst h1; simp [Core.lookup] at h2
+  case _ ih =>
+    cases wf; case _ wftl wfhd =>
+    cases wfhd;
+    simp [Functor.map, Except.map_eq_ok_iff] at h1;
+    rcases h1 with ⟨Γ', h1, h2⟩; subst G'
+    simp [Core.lookup] at h2; split at h2 <;> try simp at h2
+    replace h2 := Vec.fold_or h2
+    cases h2
+    case _ h2 =>
+      cases wf'; case _ wftl' wfhd' =>
+      replace ih := ih wftl h1 h2 wftl'; rcases ih with ⟨cls, ih⟩;
+      simp[Intermediate.lookup]; exists cls
+      split
+      contradiction
+      rw[ih]; simp [Vec.fold_or_val_eq]
+    exfalso; case _ h2 => rcases h2 with ⟨i, h2⟩; simp at h2
+  case _ ih =>  -- defn
+    cases wf; case _ wftl _ =>
+    simp [bind, Except.bind_eq_ok_iff] at h1
+    rcases h1 with ⟨Γ', h1, h3⟩
+    simp [Functor.map, Except.map_eq_ok_iff] at h3
+    rcases h3 with ⟨t', h3, h4⟩; subst G'
+    simp [Core.lookup] at h2
+    split at h2 <;> try simp at h2
     cases wf'; case _ wftl' wfhd' =>
-    replace ih := ih wftl h1 h2 wftl'; rcases ih with ⟨cls, ih⟩;
-    simp[Intermediate.lookup]; exists cls
+    replace ih := ih wftl h1 h2 wftl'; rcases ih with ⟨cls, ih⟩
+    exists cls; simp [Intermediate.lookup]
     split
     contradiction
-    rw[ih]; simp [Vec.fold_or_val_eq]
-  exfalso; case _ h2 => rcases h2 with ⟨i, h2⟩; simp at h2
-case _ ih =>  -- defn
-  cases wf; case _ wftl _ =>
-  simp [bind, Except.bind_eq_ok_iff] at h1
-  rcases h1 with ⟨Γ', h1, h3⟩
-  simp [Functor.map, Except.map_eq_ok_iff] at h3
-  rcases h3 with ⟨t', h3, h4⟩; subst G'
-  simp [Core.lookup] at h2
-  split at h2 <;> try simp at h2
-  cases wf'; case _ wftl' wfhd' =>
-  replace ih := ih wftl h1 h2 wftl'; rcases ih with ⟨cls, ih⟩
-  exists cls; simp [Intermediate.lookup]
-  split
-  contradiction
-  apply ih
-case _ cls_name _ _ _ _ _ ih => -- openm
-  cases wf; case _ wftl wfhd =>
-  simp [Functor.map, Except.map_eq_ok_iff] at h1;
-  rcases h1 with ⟨Γ', h1, h2⟩; subst G'
-  replace h2 := Core.lookup_append_some wf' h2
-  cases h2
-  case _ h2 =>
+    apply ih
+  case _ cls_name _ _ _ _ _ ih => -- openm
+    cases wf; case _ wftl wfhd =>
+    simp [Functor.map, Except.map_eq_ok_iff] at h1;
+    rcases h1 with ⟨Γ', h1, h2⟩; subst G'
+    replace h2 := Core.lookup_append_some wf' h2
+    cases h2
+    case _ h2 =>
 
+      sorry
+    case _ h2 =>
+      sorry
+
+    -- cases wf; case _ wf wfhd =>
+    -- rw[Option.bind_eq_some_iff] at h1; rcases h1 with ⟨Γ', h3, h1⟩
+    -- simp at h1; subst G'
+    -- replace h2 := Core.lookup_append h2
+    -- cases h2
+    -- case _ h2 =>
+    --   replace h2 := Core.lookup_append h2
+    --   cases h2
+    --   case _ h2 =>
+    --     simp at h2;
+    --     exists cls_name
+    --     cases wfhd; simp[Intermediate.lookup];
+    --     split;
+    --     · exfalso; sorry
+    --     · split
+    --       · exfalso; sorry
+    --       · split
+    --         case _ h _ _ _ h' =>
+    --           simp; rw[List.findIdx?_eq_some_iff_getElem] at h;
+    --           simp at h; rcases h with ⟨h1, h2, h3⟩
+    --           rw[List.getElem?_eq_getElem h1] at h'; simp at h'
+    --           subst mn; rw[h']; simp;
+    --           sorry
+    --         case _ h _ h' =>
+    --           exfalso
+    --           rw[List.findIdx?_eq_some_iff_getElem] at h;
+    --           simp at h; rcases h with ⟨h1, h2, h3⟩
+    --           rw[List.getElem?_eq_getElem h1] at h'; simp at h'
+    --   case _ h2 => simp [Core.lookup] at h2
+    -- case _ h2 =>
+    --   rcases h2 with ⟨_, h2⟩
+    --   replace ih := ih wf h3 h2
+    --   rcases ih with ⟨cls, ih⟩
+    --   exists cls;
+
+  case _ cls_name _ _ _ _ _ _ _ _ _ _ ih => -- inst
+    simp[bind, Except.bind_eq_ok_iff] at h1; rcases h1 with ⟨Γ', h3, h1⟩
+    simp [Functor.map, Except.map] at h1
+    repeat (split at h1 <;> simp at h1)
+    -- simp at h1;
+    subst G'
+    case _ h1 =>
+    cases wf; case _ wftl wfhd =>
+    replace ih := @ih mn _ wftl h3
+    cases wfhd;
+    -- replace h2 := Core.lookup_append wf h2
+    -- cases h2
+    -- case _ h2 =>
+    --   cases wfhd;
+    --   exfalso
+    --   replace h2 := Core.lookup_append h2
+    --   cases h2
+    --   case _ h2 => apply mk_inst_mths_IC_lookup h1 h2
+    --   case _ h2 => rcases h2 with ⟨e, h2⟩; simp [Core.lookup] at h2
+    -- case _ h2 =>
+    --   rcases h2 with ⟨h2, h5⟩
+    --   replace ih := ih h5; rcases ih with ⟨cls, ih⟩
+    --   exists cls; simp [Intermediate.lookup];
+    --   split
+    --   case _ e =>
+    --     exfalso; subst e; cases wfhd; case _ lk _ _ _ => rw[lk] at ih; simp at ih
+    --   apply ih
     sorry
-  case _ h2 =>
-    sorry
-
-  -- cases wf; case _ wf wfhd =>
-  -- rw[Option.bind_eq_some_iff] at h1; rcases h1 with ⟨Γ', h3, h1⟩
-  -- simp at h1; subst G'
-  -- replace h2 := Core.lookup_append h2
-  -- cases h2
-  -- case _ h2 =>
-  --   replace h2 := Core.lookup_append h2
-  --   cases h2
-  --   case _ h2 =>
-  --     simp at h2;
-  --     exists cls_name
-  --     cases wfhd; simp[Intermediate.lookup];
-  --     split;
-  --     · exfalso; sorry
-  --     · split
-  --       · exfalso; sorry
-  --       · split
-  --         case _ h _ _ _ h' =>
-  --           simp; rw[List.findIdx?_eq_some_iff_getElem] at h;
-  --           simp at h; rcases h with ⟨h1, h2, h3⟩
-  --           rw[List.getElem?_eq_getElem h1] at h'; simp at h'
-  --           subst mn; rw[h']; simp;
-  --           sorry
-  --         case _ h _ h' =>
-  --           exfalso
-  --           rw[List.findIdx?_eq_some_iff_getElem] at h;
-  --           simp at h; rcases h with ⟨h1, h2, h3⟩
-  --           rw[List.getElem?_eq_getElem h1] at h'; simp at h'
-  --   case _ h2 => simp [Core.lookup] at h2
-  -- case _ h2 =>
-  --   rcases h2 with ⟨_, h2⟩
-  --   replace ih := ih wf h3 h2
-  --   rcases ih with ⟨cls, ih⟩
-  --   exists cls;
-
-case _ cls_name _ _ _ _ _ _ _ _ _ _ ih => -- inst
-  simp[bind, Except.bind_eq_ok_iff] at h1; rcases h1 with ⟨Γ', h3, h1⟩
-  simp [Functor.map, Except.map] at h1
-  repeat (split at h1 <;> simp at h1)
-  -- simp at h1;
-  subst G'
-  case _ h1 =>
-  cases wf; case _ wftl wfhd =>
-  replace ih := @ih mn _ wftl h3
-  cases wfhd;
-  -- replace h2 := Core.lookup_append wf h2
-  -- cases h2
-  -- case _ h2 =>
-  --   cases wfhd;
-  --   exfalso
-  --   replace h2 := Core.lookup_append h2
-  --   cases h2
-  --   case _ h2 => apply mk_inst_mths_IC_lookup h1 h2
-  --   case _ h2 => rcases h2 with ⟨e, h2⟩; simp [Core.lookup] at h2
-  -- case _ h2 =>
-  --   rcases h2 with ⟨h2, h5⟩
-  --   replace ih := ih h5; rcases ih with ⟨cls, ih⟩
-  --   exists cls; simp [Intermediate.lookup];
-  --   split
-  --   case _ e =>
-  --     exfalso; subst e; cases wfhd; case _ lk _ _ _ => rw[lk] at ih; simp at ih
-  --   apply ih
-  sorry
 
 theorem translate_IC_sound {G : Intermediate.GlobalEnv} {G' : Core.GlobalEnv} (wf : ⊢ G):
   Ω G ->
   ⟦ G ⟧ = .ok G' ->
-  Ω G' := by
-intro oe h1
-intro x na nb nc Ks1 Ks2 Ts R q h2 h3
-have lem1 := translate_IC_lookup_openm wf h1 h2
-have lem2 := translate_IC_query wf h1 h3
-rcases lem1 with ⟨cls, lem1⟩
-replace oe := @oe x na nb nc Ks1 Ks2 Ts R q cls lem1 lem2
-rcases oe with ⟨i, n, cls_name, k1, k2, k3, Ks1, Ks2, tys, fds, scs, mths, oe1, j, oe2⟩
-cases oe2
-case _ oe2 => sorry
-case _ oe2 =>
+  Ω G'
+:= by
+  intro oe h1
+  intro x na nb nc Ks1 Ks2 Ts R q h2 h3
+  have lem1 := translate_IC_lookup_openm wf h1 h2
+  have lem2 := translate_IC_query wf h1 h3
+  rcases lem1 with ⟨cls, lem1⟩
+  replace oe := @oe x na nb nc Ks1 Ks2 Ts R q cls lem1 lem2
+  rcases oe with ⟨i, n, cls_name, k1, k2, k3, Ks1, Ks2, tys, fds, scs, mths, oe1, j, oe2⟩
   cases oe2
   case _ oe2 => sorry
   case _ oe2 =>
-   have lem := translate_IC_indexing_inst_mths (i := i) wf h1 oe1 oe2
-   apply lem
+    cases oe2
+    case _ oe2 => sorry
+    case _ oe2 =>
+    have lem := translate_IC_indexing_inst_mths (i := i) wf h1 oe1 oe2
+    apply lem
 
 
 
@@ -1121,11 +1172,12 @@ case _ oe2 =>
 theorem translate_open_exhaustive_sound {G : Surface.GlobalEnv} {G' : Intermediate.GlobalEnv} {G'' : Core.GlobalEnv} (wf : ⊢ G) :
   ⟦ G ⟧ = .ok G' ->
   ⟦ G' ⟧ = .ok G'' ->
-  Ω G'' := by
-intro h1 h2
-have lem : Ω G' := translate_SI_sound wf h1
-have wf' : ⊢ G' := translate_SI_wf_sound wf h1
-have lem2 : Ω G'' := translate_IC_sound wf' lem h2
-apply lem2
+  Ω G''
+:= by
+  intro h1 h2
+  have lem : Ω G' := translate_SI_sound wf h1
+  have wf' : ⊢ G' := translate_SI_wf_sound wf h1
+  have lem2 : Ω G'' := translate_IC_sound wf' lem h2
+  apply lem2
 
 end Translation
